proof/amd64/avx2/Keccak1600_array_avx2.ec
@@ -1,0 +1,1208 @@
+(******************************************************************************
+   Keccak1600_array_avx2.ec:
+
+   Correctness proof for the Keccak (fixed-sized) array based
+  absorb/squeeze AVX2 implementation
+
+
+
+******************************************************************************)
+
+require import List Real Distr Int IntDiv StdOrder Ring.
+
+import IntID.
+
+from Jasmin require import JModel.
+from Jasmin require import JArray.
+
+from CryptoSpecs require import FIPS202_SHA3.
+from CryptoSpecs require export Keccak1600_Spec Keccakf1600_Spec.
+
+from JazzEC require import WArray200.
+from JazzEC require Jazz_avx2.
+
+require import Array4 Array5 Array7 Array24 Array25.
+
+from CryptoSpecs require import FIPS202_Keccakf1600.
+from CryptoSpecs require import Keccakf1600_Spec.
+
+require import Keccak1600_avx2 Keccak1600_imem_avx2.
+
+abstract theory KeccakAvx2.
+
+op aSIZE: int.
+axiom aSIZE_ge0: 0 <= aSIZE.
+
+module type MParam = {
+  proc keccakf1600_avx2 (st:W256.t Array7.t) : W256.t Array7.t
+  proc state_init_avx2 () : W256.t Array7.t
+  proc pstate_init_avx2 (pst:W64.t Array25.t) : W64.t Array25.t
+  proc addratebit_avx2 (st:W256.t Array7.t, rATE8:int) : W256.t Array7.t
+  proc addstate_r3456_avx2 (st:W256.t Array7.t, r3 r4 r5 r6: W256.t): W256.t Array7.t
+  proc addpst01_avx2 (st: W256.t Array7.t, pst: W64.t Array25.t): W256.t Array7.t
+  proc addpstate_avx2 (st: W256.t Array7.t, pst:W64.t Array25.t): W256.t Array7.t 
+}.
+
+clone import PolyArray as A
+ with op size <= aSIZE
+      proof ge0_size by exact aSIZE_ge0.
+
+clone import WArray as WA
+ with op size <= aSIZE.
+
+module M(P: MParam) = {
+  proc __aread_subu64 (buf:W8.t A.t, offset:W64.t, dELTA:int, lEN:int,
+                       tRAIL:int) : int * int * int * W64.t = {
+    var w:W64.t;
+    var iLEN:int;
+    var t16:W64.t;
+    var t8:W64.t;
+    iLEN <- lEN;
+    if ((lEN <= 0)) {
+      w <- (W64.of_int (tRAIL %% 256));
+      tRAIL <- 0;
+    } else {
+      if ((8 <= lEN)) {
+        w <-
+        (get64_direct (WA.init8 (fun i => buf.[i]))
+        (W64.to_uint (offset + (W64.of_int dELTA))));
+        dELTA <- (dELTA + 8);
+        lEN <- (lEN - 8);
+      } else {
+        if ((4 <= lEN)) {
+          w <-
+          (zeroextu64
+          (get32_direct (WA.init8 (fun i => buf.[i]))
+          (W64.to_uint (offset + (W64.of_int dELTA)))));
+          dELTA <- (dELTA + 4);
+          lEN <- (lEN - 4);
+        } else {
+          w <- (W64.of_int 0);
+        }
+        if ((2 <= lEN)) {
+          t16 <-
+          (zeroextu64
+          (get16_direct (WA.init8 (fun i => buf.[i]))
+          (W64.to_uint (offset + (W64.of_int dELTA)))));
+          dELTA <- (dELTA + 2);
+          lEN <- (lEN - 2);
+        } else {
+          t16 <- (W64.of_int 0);
+        }
+        if (((1 <= lEN) \/ ((tRAIL %% 256) <> 0))) {
+          if ((1 <= lEN)) {
+            t8 <-
+            (zeroextu64
+            (get8_direct (WA.init8 (fun i => buf.[i]))
+            (W64.to_uint (offset + (W64.of_int dELTA)))));
+            if (((tRAIL %% 256) <> 0)) {
+              t8 <- (t8 `|` (W64.of_int (256 * (tRAIL %% 256))));
+            } else {
+              
+            }
+            dELTA <- (dELTA + 1);
+            lEN <- (lEN - 1);
+          } else {
+            t8 <- (W64.of_int (tRAIL %% 256));
+          }
+          tRAIL <- 0;
+          t8 <- (t8 `<<` (W8.of_int (8 * (2 * ((iLEN %/ 2) %% 2)))));
+          t16 <- (t16 `|` t8);
+        } else {
+          
+        }
+        t16 <- (t16 `<<` (W8.of_int (8 * (4 * ((iLEN %/ 4) %% 2)))));
+        w <- (w `|` t16);
+      }
+    }
+    return (dELTA, lEN, tRAIL, w);
+  }
+  proc __aread_bcast_4subu64 (buf:W8.t A.t, offset:W64.t, dELTA:int,
+                              lEN:int, tRAIL:int) : int * int * int * W256.t = {
+    var w:W256.t;
+    var t64:W64.t;
+    var t128:W128.t;
+    if (((lEN <= 0) /\ ((tRAIL %% 256) = 0))) {
+      w <- (set0_256);
+    } else {
+      if ((8 <= lEN)) {
+        w <-
+        (VPBROADCAST_4u64
+        (get64_direct (WA.init8 (fun i => buf.[i]))
+        (W64.to_uint (offset + (W64.of_int dELTA)))));
+        dELTA <- (dELTA + 8);
+        lEN <- (lEN - 8);
+      } else {
+        (dELTA, lEN, tRAIL, t64) <@ __aread_subu64 (buf, offset, dELTA, 
+        lEN, tRAIL);
+        t128 <- (zeroextu128 t64);
+        w <- (VPBROADCAST_4u64 (truncateu64 t128));
+      }
+    }
+    return (dELTA, lEN, tRAIL, w);
+  }
+  proc __aread_subu128 (buf:W8.t A.t, offset:W64.t, dELTA:int,
+                        lEN:int, tRAIL:int) : int * int * int * W128.t = {
+    var w:W128.t;
+    var t64:W64.t;
+    if (((lEN <= 0) /\ ((tRAIL %% 256) = 0))) {
+      w <- (set0_128);
+    } else {
+      if ((16 <= lEN)) {
+        w <-
+        (get128_direct (WA.init8 (fun i => buf.[i]))
+        (W64.to_uint (offset + (W64.of_int dELTA))));
+        dELTA <- (dELTA + 16);
+        lEN <- (lEN - 16);
+      } else {
+        if ((8 <= lEN)) {
+          w <-
+          (VMOV_64
+          (get64_direct (WA.init8 (fun i => buf.[i]))
+          (W64.to_uint (offset + (W64.of_int dELTA)))));
+          dELTA <- (dELTA + 8);
+          lEN <- (lEN - 8);
+          (dELTA, lEN, tRAIL, t64) <@ __aread_subu64 (buf, offset, dELTA,
+          lEN, tRAIL);
+          w <- (VPINSR_2u64 w t64 (W8.of_int 1));
+        } else {
+          (dELTA, lEN, tRAIL, t64) <@ __aread_subu64 (buf, offset, dELTA,
+          lEN, tRAIL);
+          w <- (zeroextu128 t64);
+        }
+      }
+    }
+    return (dELTA, lEN, tRAIL, w);
+  }
+  proc __aread_subu256 (buf:W8.t A.t, offset:W64.t, dELTA:int,
+                        lEN:int, tRAIL:int) : int * int * int * W256.t = {
+    var w:W256.t;
+    var t128_1:W128.t;
+    var t128_0:W128.t;
+    if (((lEN <= 0) /\ ((tRAIL %% 256) = 0))) {
+      w <- (set0_256);
+    } else {
+      if ((32 <= lEN)) {
+        w <-
+        (get256_direct (WA.init8 (fun i => buf.[i]))
+        (W64.to_uint (offset + (W64.of_int dELTA))));
+        dELTA <- (dELTA + 32);
+        lEN <- (lEN - 32);
+      } else {
+        if ((16 <= lEN)) {
+          t128_0 <-
+          (get128_direct (WA.init8 (fun i => buf.[i]))
+          (W64.to_uint (offset + (W64.of_int dELTA))));
+          dELTA <- (dELTA + 16);
+          lEN <- (lEN - 16);
+          (dELTA, lEN, tRAIL, t128_1) <@ __aread_subu128 (buf, offset, 
+          dELTA, lEN, tRAIL);
+          w <-
+          (W256.of_int
+          (((W128.to_uint t128_0) %% (2 ^ 128)) +
+          ((2 ^ 128) * (W128.to_uint t128_1))));
+        } else {
+          t128_1 <- (set0_128);
+          (dELTA, lEN, tRAIL, t128_0) <@ __aread_subu128 (buf, offset, 
+          dELTA, lEN, tRAIL);
+          w <-
+          (W256.of_int
+          (((W128.to_uint t128_0) %% (2 ^ 128)) +
+          ((2 ^ 128) * (W128.to_uint t128_1))));
+        }
+      }
+    }
+    return (dELTA, lEN, tRAIL, w);
+  }
+  proc __awrite_subu64 (buf:W8.t A.t, offset:W64.t, dELTA:int,
+                        lEN:int, w:W64.t) : W8.t A.t * int * int = {
+    
+    if ((0 < lEN)) {
+      if ((8 <= lEN)) {
+        buf <-
+        (A.init
+        (WA.get8
+        (WA.set64_direct (WA.init8 (fun i => buf.[i]))
+        (W64.to_uint (offset + (W64.of_int dELTA))) w)));
+        dELTA <- (dELTA + 8);
+        lEN <- (lEN - 8);
+      } else {
+        if ((4 <= lEN)) {
+          buf <-
+          (A.init
+          (WA.get8
+          (WA.set32_direct (WA.init8 (fun i => buf.[i]))
+          (W64.to_uint (offset + (W64.of_int dELTA))) (truncateu32 w))));
+          w <- (w `>>` (W8.of_int 32));
+          dELTA <- (dELTA + 4);
+          lEN <- (lEN - 4);
+        } else {
+          
+        }
+        if ((2 <= lEN)) {
+          buf <-
+          (A.init
+          (WA.get8
+          (WA.set16_direct (WA.init8 (fun i => buf.[i]))
+          (W64.to_uint (offset + (W64.of_int dELTA))) (truncateu16 w))));
+          w <- (w `>>` (W8.of_int 16));
+          dELTA <- (dELTA + 2);
+          lEN <- (lEN - 2);
+        } else {
+          
+        }
+        if ((1 <= lEN)) {
+          buf <-
+          (A.init
+          (WA.get8
+          (WA.set8_direct (WA.init8 (fun i => buf.[i]))
+          (W64.to_uint (offset + (W64.of_int dELTA))) (truncateu8 w))));
+          dELTA <- (dELTA + 1);
+          lEN <- (lEN - 1);
+        } else {
+          
+        }
+      }
+    } else {
+      
+    }
+    return (buf, dELTA, lEN);
+  }
+  proc __awrite_subu128 (buf:W8.t A.t, offset:W64.t, dELTA:int,
+                         lEN:int, w:W128.t) : W8.t A.t * int * int = {
+    var t64:W64.t;
+    if ((0 < lEN)) {
+      if ((16 <= lEN)) {
+        buf <-
+        (A.init
+        (WA.get8
+        (WA.set128_direct (WA.init8 (fun i => buf.[i]))
+        (W64.to_uint (offset + (W64.of_int dELTA))) w)));
+        dELTA <- (dELTA + 16);
+        lEN <- (lEN - 16);
+      } else {
+        if ((8 <= lEN)) {
+          buf <-
+          (A.init
+          (WA.get8
+          (WA.set64_direct (WA.init8 (fun i => buf.[i]))
+          (W64.to_uint (offset + (W64.of_int dELTA)))
+          (MOVV_64 (truncateu64 w)))));
+          dELTA <- (dELTA + 8);
+          lEN <- (lEN - 8);
+          w <- (VPUNPCKH_2u64 w w);
+        } else {
+          
+        }
+        t64 <- (truncateu64 w);
+        (buf, dELTA, lEN) <@ __awrite_subu64 (buf, offset, dELTA, lEN, t64);
+      }
+    } else {
+      
+    }
+    return (buf, dELTA, lEN);
+  }
+  proc __awrite_subu256 (buf:W8.t A.t, offset:W64.t, dELTA:int,
+                         lEN:int, w:W256.t) : W8.t A.t * int * int = {
+    var t128:W128.t;
+    if ((0 < lEN)) {
+      if ((32 <= lEN)) {
+        buf <-
+        (A.init
+        (WA.get8
+        (WA.set256_direct (WA.init8 (fun i => buf.[i]))
+        (W64.to_uint (offset + (W64.of_int dELTA))) w)));
+        dELTA <- (dELTA + 32);
+        lEN <- (lEN - 32);
+      } else {
+        if ((16 <= lEN)) {
+          buf <-
+          (A.init
+          (WA.get8
+          (WA.set128_direct (WA.init8 (fun i => buf.[i]))
+          (W64.to_uint (offset + (W64.of_int dELTA))) (truncateu128 w))));
+          dELTA <- (dELTA + 16);
+          lEN <- (lEN - 16);
+          t128 <- (VEXTRACTI128 w (W8.of_int 1));
+        } else {
+          t128 <- (truncateu128 w);
+        }
+        (buf, dELTA, lEN) <@ __awrite_subu128 (buf, offset, dELTA, lEN,
+        t128);
+      }
+    } else {
+      
+    }
+    return (buf, dELTA, lEN);
+  }
+  proc __addstate_array_avx2 (st:W256.t Array7.t, buf:W8.t A.t,
+                              offset:W64.t, lEN:int, tRAILB:int) : W256.t Array7.t *
+                                                                   W64.t = {
+    var dELTA:int;
+    var t64:W64.t;
+    var t128_0:W128.t;
+    var r0:W256.t;
+    var r1:W256.t;
+    var t128_1:W128.t;
+    var r3:W256.t;
+    var r4:W256.t;
+    var r5:W256.t;
+    var r2:W256.t;
+    var r6:W256.t;
+    dELTA <- 0;
+    (dELTA, lEN, tRAILB, t64) <@ __aread_subu64 (buf, offset, dELTA, 
+    lEN, tRAILB);
+    t128_0 <- (zeroextu128 t64);
+    r0 <- (VPBROADCAST_4u64 (truncateu64 t128_0));
+    st.[0] <- (st.[0] `^` r0);
+    (dELTA, lEN, tRAILB, r1) <@ __aread_subu256 (buf, offset, dELTA, 
+    lEN, tRAILB);
+    st.[1] <- (st.[1] `^` r1);
+    if ((0 < lEN)) {
+      (dELTA, lEN, tRAILB, t64) <@ __aread_subu64 (buf, offset, dELTA, 
+      lEN, tRAILB);
+      t128_1 <- (zeroextu128 t64);
+      (dELTA, lEN, tRAILB, r3) <@ __aread_subu256 (buf, offset, dELTA, 
+      lEN, tRAILB);
+      (dELTA, lEN, tRAILB, t64) <@ __aread_subu64 (buf, offset, dELTA, 
+      lEN, tRAILB);
+      t128_0 <- (zeroextu128 t64);
+      (dELTA, lEN, tRAILB, r4) <@ __aread_subu256 (buf, offset, dELTA, 
+      lEN, tRAILB);
+      (dELTA, lEN, tRAILB, t64) <@ __aread_subu64 (buf, offset, dELTA, 
+      lEN, tRAILB);
+      t128_1 <- (VPINSR_2u64 t128_1 t64 (W8.of_int 1));
+      (dELTA, lEN, tRAILB, r5) <@ __aread_subu256 (buf, offset, dELTA, 
+      lEN, tRAILB);
+      (dELTA, lEN, tRAILB, t64) <@ __aread_subu64 (buf, offset, dELTA, 
+      lEN, tRAILB);
+      t128_0 <- (VPINSR_2u64 t128_0 t64 (W8.of_int 1));
+      r2 <-
+      (W256.of_int
+      (((W128.to_uint t128_0) %% (2 ^ 128)) +
+      ((2 ^ 128) * (W128.to_uint t128_1))));
+      st.[2] <- (st.[2] `^` r2);
+      (dELTA, lEN, tRAILB, r6) <@ __aread_subu256 (buf, offset, dELTA, 
+      lEN, tRAILB);
+      st <@ P.addstate_r3456_avx2 (st, r3, r4, r5, r6);
+    } else {
+      
+    }
+    offset <- (offset + (W64.of_int dELTA));
+    return (st, offset);
+  }
+  proc __absorb_array_avx2 (st:W256.t Array7.t, buf:W8.t A.t,
+                            offset:W64.t, lEN:int, rATE8:int, tRAILB:int) : 
+  W256.t Array7.t * W64.t = {
+    var aLL:int;
+    var iTERS:int;
+    var i:W64.t;
+    aLL <- (lEN + ((tRAILB <> 0) ? 1 : 0));
+    iTERS <- (lEN %/ rATE8);
+    if ((0 < iTERS)) {
+      i <- (W64.of_int 0);
+      while ((i \ult (W64.of_int iTERS))) {
+        (st, offset) <@ __addstate_array_avx2 (st, buf, offset, rATE8, 0);
+        st <@ P.keccakf1600_avx2 (st);
+        i <- (i + (W64.of_int 1));
+      }
+    } else {
+      
+    }
+    lEN <- (lEN %% rATE8);
+    (st, offset) <@ __addstate_array_avx2 (st, buf, offset, lEN, tRAILB);
+    if ((tRAILB <> 0)) {
+      st <@ P.addratebit_avx2 (st, rATE8);
+    } else {
+      
+    }
+    return (st, offset);
+  }
+  proc __pstate_array_avx2 (pst:W64.t Array25.t, aT:int, buf:W8.t A.t,
+                            offset:W64.t, lEN:int, tRAILB:int) : W64.t Array25.t *
+                                                                 int * W64.t = {
+    var aLL:int;
+    var dELTA:int;
+    var lO:int;
+    var at:W64.t;
+    var t64:W64.t;
+    var t256:W256.t;
+    var t128:W128.t;
+    var  _0:int;
+    var  _1:int;
+    var  _2:int;
+    var  _3:int;
+    dELTA <- 0;
+    aLL <- (aT + lEN);
+    lO <- (aT %% 8);
+    at <- (W64.of_int (aT %/ 8));
+    if ((0 < lO)) {
+      if (((lO + lEN) < 8)) {
+        if ((tRAILB <> 0)) {
+          aLL <- (aLL + 1);
+        } else {
+          
+        }
+        (dELTA,  _2, tRAILB, t64) <@ __aread_subu64 (buf, offset, dELTA, 
+        lEN, tRAILB);
+        t64 <- (t64 `<<` (W8.of_int (8 * lO)));
+        pst.[(W64.to_uint at)] <- (pst.[(W64.to_uint at)] `^` t64);
+        lO <- 0;
+        aT <- 0;
+        lEN <- 0;
+      } else {
+        if ((8 <= lEN)) {
+          t64 <-
+          (get64_direct (WA.init8 (fun i => buf.[i]))
+          (W64.to_uint (offset + (W64.of_int dELTA))));
+          dELTA <- (dELTA + (8 - lO));
+        } else {
+          (dELTA,  _0,  _1, t64) <@ __aread_subu64 (buf, offset, dELTA,
+          (8 - lO), 0);
+        }
+        lEN <- (lEN - (8 - lO));
+        aT <- (aT + (8 - lO));
+        t64 <- (t64 `<<` (W8.of_int (8 * lO)));
+        pst.[(W64.to_uint at)] <- (pst.[(W64.to_uint at)] `^` t64);
+        at <- (at + (W64.of_int 1));
+      }
+    } else {
+      
+    }
+    if ((32 <= lEN)) {
+      offset <- (offset + (W64.of_int dELTA));
+      dELTA <- 0;
+      while ((at \ult (W64.of_int ((aT %/ 8) + (4 * (lEN %/ 32)))))) {
+        t256 <-
+        (get256_direct (WA.init8 (fun i => buf.[i]))
+        (W64.to_uint offset));
+        offset <- (offset + (W64.of_int 32));
+        pst <-
+        (Array25.init
+        (WArray200.get64
+        (WArray200.set256_direct (WArray200.init64 (fun i => pst.[i]))
+        (W64.to_uint ((W64.of_int 8) * at)) t256)));
+        at <- (at + (W64.of_int 4));
+      }
+      lEN <- (lEN %% 32);
+    } else {
+      
+    }
+    if ((16 <= lEN)) {
+      t128 <-
+      (get128_direct (WA.init8 (fun i => buf.[i]))
+      (W64.to_uint (offset + (W64.of_int dELTA))));
+      dELTA <- (dELTA + 16);
+      pst <-
+      (Array25.init
+      (WArray200.get64
+      (WArray200.set128_direct (WArray200.init64 (fun i => pst.[i]))
+      (W64.to_uint ((W64.of_int 8) * at)) t128)));
+      at <- (at + (W64.of_int 2));
+      lEN <- (lEN - 16);
+    } else {
+      
+    }
+    if ((8 <= lEN)) {
+      t64 <-
+      (get64_direct (WA.init8 (fun i => buf.[i]))
+      (W64.to_uint (offset + (W64.of_int dELTA))));
+      dELTA <- (dELTA + 8);
+      pst <-
+      (Array25.init
+      (WArray200.get64
+      (WArray200.set64_direct (WArray200.init64 (fun i => pst.[i]))
+      (W64.to_uint ((W64.of_int 8) * at)) t64)));
+      at <- (at + (W64.of_int 1));
+      lEN <- (lEN - 8);
+    } else {
+      
+    }
+    lO <- ((aT + lEN) %% 8);
+    if (((0 < lO) \/ (tRAILB <> 0))) {
+      if ((tRAILB <> 0)) {
+        aLL <- (aLL + 1);
+      } else {
+        
+      }
+      (dELTA,  _3, tRAILB, t64) <@ __aread_subu64 (buf, offset, dELTA, 
+      lO, tRAILB);
+      pst.[(aLL %/ 8)] <- t64;
+    } else {
+      
+    }
+    offset <- (offset + (W64.of_int dELTA));
+    return (pst, aLL, offset);
+  }
+  proc __pabsorb_array_avx2 (pst:W64.t Array25.t, aT:int, st:W256.t Array7.t,
+                             buf:W8.t A.t, offset:W64.t, lEN:int,
+                             rATE8:int, tRAILB:int) : W64.t Array25.t * int *
+                                                      W256.t Array7.t * W64.t = {
+    var aLL:int;
+    var iTERS:int;
+    var i:W64.t;
+    var  _0:int;
+    aLL <- (aT + lEN);
+    if (((aT + lEN) < rATE8)) {
+      (pst, aT, offset) <@ __pstate_array_avx2 (pst, aT, buf, offset, 
+      lEN, tRAILB);
+      if ((tRAILB <> 0)) {
+        i <- (W64.of_int ((aT %/ 8) + 1));
+        if ((aT <= (5 * 8))) {
+          while ((i \ult (W64.of_int 5))) {
+            pst.[(W64.to_uint i)] <- (W64.of_int 0);
+            i <- (i + (W64.of_int 1));
+          }
+          st <@ P.addpst01_avx2 (st, pst);
+          st <@ P.addratebit_avx2 (st, rATE8);
+        } else {
+          while ((i \ult (W64.of_int (rATE8 %/ 8)))) {
+            pst.[(W64.to_uint i)] <- (W64.of_int 0);
+            i <- (i + (W64.of_int 1));
+          }
+          pst <-
+          (Array25.init
+          (WArray200.get64
+          (WArray200.set8 (WArray200.init64 (fun i_0 => pst.[i_0]))
+          (rATE8 - 1)
+          ((get8 (WArray200.init64 (fun i_0 => pst.[i_0])) (rATE8 - 1)) `^`
+          (W8.of_int 128)))));
+          st <@ P.addpstate_avx2 (st, pst);
+        }
+      } else {
+        
+      }
+    } else {
+      if ((aT <> 0)) {
+        (pst,  _0, offset) <@ __pstate_array_avx2 (pst, aT, buf, offset,
+        (rATE8 - aT), 0);
+        lEN <- (lEN - (rATE8 - aT));
+        st <@ P.addpstate_avx2 (st, pst);
+        st <@ P.keccakf1600_avx2 (st);
+        aT <- 0;
+      } else {
+        
+      }
+      iTERS <- (lEN %/ rATE8);
+      i <- (W64.of_int 0);
+      while ((i \ult (W64.of_int iTERS))) {
+        (st, offset) <@ __addstate_array_avx2 (st, buf, offset, rATE8, 0);
+        st <@ P.keccakf1600_avx2 (st);
+        i <- (i + (W64.of_int 1));
+      }
+      lEN <- (aLL %% rATE8);
+      if ((tRAILB <> 0)) {
+        (st, offset) <@ __addstate_array_avx2 (st, buf, offset, lEN, tRAILB);
+        st <@ P.addratebit_avx2 (st, rATE8);
+      } else {
+        if ((lEN <> 0)) {
+          (pst, aT, offset) <@ __pstate_array_avx2 (pst, 0, buf, offset, 
+          lEN, tRAILB);
+        } else {
+          
+        }
+      }
+    }
+    return (pst, aT, st, offset);
+  }
+  proc __dumpstate_array_avx2 (buf:W8.t A.t, offset:W64.t, lEN:int,
+                               st:W256.t Array7.t) : W8.t A.t * W64.t = {
+    var dELTA:int;
+    var t128_0:W128.t;
+    var t128_1:W128.t;
+    var t:W64.t;
+    var t256_0:W256.t;
+    var t256_1:W256.t;
+    var t256_2:W256.t;
+    var t256_3:W256.t;
+    var t256_4:W256.t;
+    var  _0:int;
+    dELTA <- 0;
+    if ((8 <= lEN)) {
+      (buf, dELTA,  _0) <@ __awrite_subu256 (buf, offset, dELTA, 8, st.[0]);
+      lEN <- (lEN - 8);
+    } else {
+      (buf, dELTA, lEN) <@ __awrite_subu256 (buf, offset, dELTA, lEN,
+      st.[0]);
+    }
+    (buf, dELTA, lEN) <@ __awrite_subu256 (buf, offset, dELTA, lEN, st.[1]);
+    if ((0 < lEN)) {
+      t128_0 <- (truncateu128 st.[2]);
+      t128_1 <- (VEXTRACTI128 st.[2] (W8.of_int 1));
+      t <- (truncateu64 t128_1);
+      (buf, dELTA, lEN) <@ __awrite_subu64 (buf, offset, dELTA, lEN, t);
+      t128_1 <- (VPUNPCKH_2u64 t128_1 t128_1);
+    } else {
+      
+    }
+    if ((0 < lEN)) {
+      t256_0 <-
+      (VPBLEND_8u32 st.[3] st.[4]
+      (W8.of_int
+      ((0 %% (2 ^ 1)) +
+      ((2 ^ 1) *
+      ((0 %% (2 ^ 1)) +
+      ((2 ^ 1) *
+      ((0 %% (2 ^ 1)) +
+      ((2 ^ 1) *
+      ((0 %% (2 ^ 1)) +
+      ((2 ^ 1) *
+      ((1 %% (2 ^ 1)) +
+      ((2 ^ 1) *
+      ((1 %% (2 ^ 1)) + ((2 ^ 1) * ((1 %% (2 ^ 1)) + ((2 ^ 1) * 1))))))))))))))
+      ));
+      t256_1 <-
+      (VPBLEND_8u32 st.[4] st.[3]
+      (W8.of_int
+      ((0 %% (2 ^ 1)) +
+      ((2 ^ 1) *
+      ((0 %% (2 ^ 1)) +
+      ((2 ^ 1) *
+      ((0 %% (2 ^ 1)) +
+      ((2 ^ 1) *
+      ((0 %% (2 ^ 1)) +
+      ((2 ^ 1) *
+      ((1 %% (2 ^ 1)) +
+      ((2 ^ 1) *
+      ((1 %% (2 ^ 1)) + ((2 ^ 1) * ((1 %% (2 ^ 1)) + ((2 ^ 1) * 1))))))))))))))
+      ));
+      t256_2 <-
+      (VPBLEND_8u32 st.[5] st.[6]
+      (W8.of_int
+      ((0 %% (2 ^ 1)) +
+      ((2 ^ 1) *
+      ((0 %% (2 ^ 1)) +
+      ((2 ^ 1) *
+      ((0 %% (2 ^ 1)) +
+      ((2 ^ 1) *
+      ((0 %% (2 ^ 1)) +
+      ((2 ^ 1) *
+      ((1 %% (2 ^ 1)) +
+      ((2 ^ 1) *
+      ((1 %% (2 ^ 1)) + ((2 ^ 1) * ((1 %% (2 ^ 1)) + ((2 ^ 1) * 1))))))))))))))
+      ));
+      t256_3 <-
+      (VPBLEND_8u32 st.[6] st.[5]
+      (W8.of_int
+      ((0 %% (2 ^ 1)) +
+      ((2 ^ 1) *
+      ((0 %% (2 ^ 1)) +
+      ((2 ^ 1) *
+      ((0 %% (2 ^ 1)) +
+      ((2 ^ 1) *
+      ((0 %% (2 ^ 1)) +
+      ((2 ^ 1) *
+      ((1 %% (2 ^ 1)) +
+      ((2 ^ 1) *
+      ((1 %% (2 ^ 1)) + ((2 ^ 1) * ((1 %% (2 ^ 1)) + ((2 ^ 1) * 1))))))))))))))
+      ));
+      t256_4 <-
+      (VPBLEND_8u32 t256_0 t256_3
+      (W8.of_int
+      ((1 %% (2 ^ 1)) +
+      ((2 ^ 1) *
+      ((1 %% (2 ^ 1)) +
+      ((2 ^ 1) *
+      ((0 %% (2 ^ 1)) +
+      ((2 ^ 1) *
+      ((0 %% (2 ^ 1)) +
+      ((2 ^ 1) *
+      ((0 %% (2 ^ 1)) +
+      ((2 ^ 1) *
+      ((0 %% (2 ^ 1)) + ((2 ^ 1) * ((1 %% (2 ^ 1)) + ((2 ^ 1) * 1))))))))))))))
+      ));
+      (buf, dELTA, lEN) <@ __awrite_subu256 (buf, offset, dELTA, lEN,
+      t256_4);
+      if ((0 < lEN)) {
+        t <- (truncateu64 t128_0);
+        (buf, dELTA, lEN) <@ __awrite_subu64 (buf, offset, dELTA, lEN, t);
+        t128_0 <- (VPUNPCKH_2u64 t128_0 t128_0);
+      } else {
+        
+      }
+      if ((0 < lEN)) {
+        t256_4 <-
+        (VPBLEND_8u32 t256_3 t256_1
+        (W8.of_int
+        ((1 %% (2 ^ 1)) +
+        ((2 ^ 1) *
+        ((1 %% (2 ^ 1)) +
+        ((2 ^ 1) *
+        ((0 %% (2 ^ 1)) +
+        ((2 ^ 1) *
+        ((0 %% (2 ^ 1)) +
+        ((2 ^ 1) *
+        ((0 %% (2 ^ 1)) +
+        ((2 ^ 1) *
+        ((0 %% (2 ^ 1)) + ((2 ^ 1) * ((1 %% (2 ^ 1)) + ((2 ^ 1) * 1))))))))))))))
+        ));
+        (buf, dELTA, lEN) <@ __awrite_subu256 (buf, offset, dELTA, lEN,
+        t256_4);
+      } else {
+        
+      }
+      if ((0 < lEN)) {
+        t <- (truncateu64 t128_1);
+        (buf, dELTA, lEN) <@ __awrite_subu64 (buf, offset, dELTA, lEN, t);
+      } else {
+        
+      }
+      if ((0 < lEN)) {
+        t256_4 <-
+        (VPBLEND_8u32 t256_2 t256_0
+        (W8.of_int
+        ((1 %% (2 ^ 1)) +
+        ((2 ^ 1) *
+        ((1 %% (2 ^ 1)) +
+        ((2 ^ 1) *
+        ((0 %% (2 ^ 1)) +
+        ((2 ^ 1) *
+        ((0 %% (2 ^ 1)) +
+        ((2 ^ 1) *
+        ((0 %% (2 ^ 1)) +
+        ((2 ^ 1) *
+        ((0 %% (2 ^ 1)) + ((2 ^ 1) * ((1 %% (2 ^ 1)) + ((2 ^ 1) * 1))))))))))))))
+        ));
+        (buf, dELTA, lEN) <@ __awrite_subu256 (buf, offset, dELTA, lEN,
+        t256_4);
+      } else {
+        
+      }
+      if ((0 < lEN)) {
+        t <- (truncateu64 t128_0);
+        (buf, dELTA, lEN) <@ __awrite_subu64 (buf, offset, dELTA, lEN, t);
+      } else {
+        
+      }
+      if ((0 < lEN)) {
+        t256_4 <-
+        (VPBLEND_8u32 t256_1 t256_2
+        (W8.of_int
+        ((1 %% (2 ^ 1)) +
+        ((2 ^ 1) *
+        ((1 %% (2 ^ 1)) +
+        ((2 ^ 1) *
+        ((0 %% (2 ^ 1)) +
+        ((2 ^ 1) *
+        ((0 %% (2 ^ 1)) +
+        ((2 ^ 1) *
+        ((0 %% (2 ^ 1)) +
+        ((2 ^ 1) *
+        ((0 %% (2 ^ 1)) + ((2 ^ 1) * ((1 %% (2 ^ 1)) + ((2 ^ 1) * 1))))))))))))))
+        ));
+        (buf, dELTA, lEN) <@ __awrite_subu256 (buf, offset, dELTA, lEN,
+        t256_4);
+      } else {
+        
+      }
+    } else {
+      
+    }
+    offset <- (offset + (W64.of_int dELTA));
+    return (buf, offset);
+  }
+  proc __squeeze_array_avx2 (buf:W8.t A.t, offset:W64.t, lEN:int,
+                             st:W256.t Array7.t, rATE8:int) : W8.t A.t *
+                                                              W256.t Array7.t = {
+    var iTERS:int;
+    var lO:int;
+    var i:W64.t;
+    iTERS <- (lEN %/ rATE8);
+    lO <- (lEN %% rATE8);
+    if ((0 < lEN)) {
+      if ((0 < iTERS)) {
+        i <- (W64.of_int 0);
+        while ((i \ult (W64.of_int iTERS))) {
+          st <@ P.keccakf1600_avx2 (st);
+          (buf, offset) <@ __dumpstate_array_avx2 (buf, offset, rATE8, st);
+          i <- (i + (W64.of_int 1));
+        }
+      } else {
+        
+      }
+      if ((0 < lO)) {
+        st <@ P.keccakf1600_avx2 (st);
+        (buf, offset) <@ __dumpstate_array_avx2 (buf, offset, lO, st);
+      } else {
+        
+      }
+    } else {
+      
+    }
+    return (buf, st);
+  }
+}.
+
+
+(*
+   PARAMETER MODULE
+*)
+module P: MParam = {
+  proc keccakf1600_avx2 = Jazz_avx2.M._keccakf1600_avx2
+  proc state_init_avx2 = Jazz_avx2.M.__state_init_avx2
+  proc pstate_init_avx2 = Jazz_avx2.M.__pstate_init_avx2
+  proc addratebit_avx2 = Jazz_avx2.M.__addratebit_avx2
+  proc addstate_r3456_avx2 = Jazz_avx2.M.__addstate_r3456_avx2
+  proc addpst01_avx2 = Jazz_avx2.M.__addpst01_avx2
+  proc addpstate_avx2 = Jazz_avx2.M._addpstate_avx2
+}.
+
+
+lemma  aread_subu64_ll: islossless M(P).__aread_subu64
+ by islossless.
+
+hoare aread_subu64_h _buf _off _dlt _len _trail:
+ M(P).__aread_subu64
+ : buf=_buf /\ offset=_off /\ dELTA=_dlt /\ lEN=_len /\ tRAIL=_trail
+ ==> res.`1 = _dlt + min (max 0 _len) 8
+  /\ res.`2 = _len - min (max 0 _len) 8
+  /\ res.`3 = (if _len < 8 then 0 else _trail)
+  /\ res.`4 = W8u8.pack8 (sub _buf (to_uint _off+_dlt) (min (max 0 _len) 8) ++ [W8.of_int _trail]).
+admitted.
+
+phoare aread_subu64_ph _buf _off _dlt _len _trail:
+ [ M(P).__aread_subu64
+ : buf=_buf /\ offset=_off /\ dELTA=_dlt /\ lEN=_len /\ tRAIL=_trail
+ ==> res.`1 = _dlt + min (max 0 _len) 8
+  /\ res.`2 = _len - min (max 0 _len) 8
+  /\ res.`3 = (if _len < 8 then 0 else _trail)
+  /\ res.`4 = W8u8.pack8 (sub _buf (to_uint _off+_dlt) (min (max 0 _len) 8) ++ [W8.of_int _trail])
+ ] = 1%r.
+proof.
+by conseq aread_subu64_ll (aread_subu64_h _buf _off _dlt _len _trail).
+qed.
+
+lemma  aread_subu128_ll: islossless M(P).__aread_subu128
+ by islossless.
+
+hoare aread_subu128_h _buf _off _dlt _len _trail:
+ M(P).__aread_subu128
+ : buf=_buf /\ offset=_off /\ dELTA=_dlt /\ lEN=_len /\ tRAIL=_trail
+ ==> res.`1 = _dlt + min (max 0 _len) 16
+  /\ res.`2 = _len - min (max 0 _len) 16
+  /\ res.`3 = (if _len < 16 then 0 else _trail)
+  /\ res.`4 = W16u8.pack16 (sub _buf (to_uint _off+_dlt) (min (max 0 _len) 16) ++ [W8.of_int _trail]).
+admitted.
+
+phoare aread_subu128_ph _buf _off _dlt _len _trail:
+ [ M(P).__aread_subu128
+ : buf=_buf /\ offset=_off /\ dELTA=_dlt /\ lEN=_len /\ tRAIL=_trail
+ ==> res.`1 = _dlt + min (max 0 _len) 16
+  /\ res.`2 = _len - min (max 0 _len) 16
+  /\ res.`3 = (if _len < 16 then 0 else _trail)
+  /\ res.`4 = W16u8.pack16 (sub _buf (to_uint _off+_dlt) (min (max 0 _len) 16) ++ [W8.of_int _trail])
+ ] = 1%r.
+proof.
+by conseq aread_subu128_ll (aread_subu128_h _buf _off _dlt _len _trail).
+qed.
+
+lemma  aread_subu256_ll: islossless M(P).__aread_subu256
+ by islossless.
+
+hoare aread_subu256_h _buf _off _dlt _len _trail:
+ M(P).__aread_subu256
+ : buf=_buf /\ offset=_off /\ dELTA=_dlt /\ lEN=_len /\ tRAIL=_trail
+ ==> res.`1 = _dlt + min (max 0 _len) 32
+  /\ res.`2 = _len - min (max 0 _len) 32
+  /\ res.`3 = (if _len < 32 then 0 else _trail)
+  /\ res.`4 = W32u8.pack32 (sub _buf (to_uint _off+_dlt) (min (max 0 _len) 32) ++ [W8.of_int _trail]).
+admitted.
+
+phoare aread_subu256_ph _buf _off _dlt _len _trail:
+ [ M(P).__aread_subu256
+ : buf=_buf /\ offset=_off /\ dELTA=_dlt /\ lEN=_len /\ tRAIL=_trail
+ ==> res.`1 = _dlt + min (max 0 _len) 32
+  /\ res.`2 = _len - min (max 0 _len) 32
+  /\ res.`3 = (if _len < 32 then 0 else _trail)
+  /\ res.`4 = W32u8.pack32 (sub _buf (to_uint _off+_dlt) (min (max 0 _len) 32) ++ [W8.of_int _trail])
+ ] = 1%r.
+proof.
+by conseq aread_subu256_ll (aread_subu256_h _buf _off _dlt _len _trail).
+qed.
+
+
+lemma awrite_subu64_ll: islossless M(P).__awrite_subu64
+ by islossless.
+
+hoare awrite_subu64_h _buf _off _dlt _len _w:
+ M(P).__awrite_subu64
+ : buf=_buf /\ offset=_off /\ dELTA=_dlt /\ lEN=_len
+ ==> res.`1 = A.fill (nth W8.zero (W8u8.to_list _w)) (to_uint _off + _dlt) (min (max 0 _len) 8) _buf
+  /\ res.`2 = _dlt + min (max 0 _len) 8
+  /\ res.`3 = _len - min (max 0 _len) 8.
+proof.
+admitted.
+
+phoare awrite_subu64_ph _buf _off _dlt _len _w:
+ [ M(P).__awrite_subu64
+ : buf=_buf /\ offset=_off /\ dELTA=_dlt /\ lEN=_len
+ ==> res.`1 = A.fill (nth W8.zero (W8u8.to_list _w)) (to_uint _off + _dlt) (min (max 0 _len) 8) _buf
+  /\ res.`2 = _dlt + min (max 0 _len) 8
+  /\ res.`3 = _len - min (max 0 _len) 8
+ ] = 1%r.
+proof.
+by conseq awrite_subu64_ll (awrite_subu64_h _buf _off _dlt _len _w).
+qed.
+
+lemma awrite_subu128_ll: islossless M(P).__awrite_subu128
+ by islossless.
+
+hoare awrite_subu128_h _buf _off _dlt _len _w:
+ M(P).__awrite_subu128
+ : buf=_buf /\ offset=_off /\ dELTA=_dlt /\ lEN=_len
+ ==> res.`1 = A.fill (nth W8.zero (W16u8.to_list _w)) (to_uint _off + _dlt) (min (max 0 _len) 16) _buf
+  /\ res.`2 = _dlt + min (max 0 _len) 16
+  /\ res.`3 = _len - min (max 0 _len) 16.
+proof.
+admitted.
+
+phoare awrite_subu128_ph _buf _off _dlt _len _w:
+ [ M(P).__awrite_subu128
+ : buf=_buf /\ offset=_off /\ dELTA=_dlt /\ lEN=_len
+ ==> res.`1 = A.fill (nth W8.zero (W16u8.to_list _w)) (to_uint _off + _dlt) (min (max 0 _len) 16) _buf
+  /\ res.`2 = _dlt + min (max 0 _len) 16
+  /\ res.`3 = _len - min (max 0 _len) 16
+ ] = 1%r.
+proof.
+by conseq awrite_subu128_ll (awrite_subu128_h _buf _off _dlt _len _w).
+qed.
+
+lemma awrite_subu256_ll: islossless M(P).__awrite_subu256
+ by islossless.
+
+hoare awrite_subu256_h _buf _off _dlt _len _w:
+ M(P).__awrite_subu256
+ : buf=_buf /\ offset=_off /\ dELTA=_dlt /\ lEN=_len
+ ==> res.`1 = A.fill (nth W8.zero (W32u8.to_list _w)) (to_uint _off + _dlt) (min (max 0 _len) 32) _buf
+  /\ res.`2 = _dlt + min (max 0 _len) 32
+  /\ res.`3 = _len - min (max 0 _len) 32.
+proof.
+admitted.
+
+phoare awrite_subu256_ph _buf _off _dlt _len _w:
+ [ M(P).__awrite_subu256
+ : buf=_buf /\ offset=_off /\ dELTA=_dlt /\ lEN=_len
+ ==> res.`1 = A.fill (nth W8.zero (W32u8.to_list _w)) (to_uint _off + _dlt) (min (max 0 _len) 32) _buf
+  /\ res.`2 = _dlt + min (max 0 _len) 32
+  /\ res.`3 = _len - min (max 0 _len) 32
+ ] = 1%r.
+proof.
+by conseq awrite_subu256_ll (awrite_subu256_h _buf _off _dlt _len _w).
+qed.
+
+(*
+   ONE-SHOT (FIXED-SIZE) MEMORY ABSORB
+   ===================================
+*)
+
+(*
+addstate_array_avx2
+*)
+lemma addstate_array_avx2_ll: islossless M(P).__addstate_array_avx2
+ by islossless.
+
+op addstavx2 (st: W256.t Array7.t, l: W8.t list): W256.t Array7.t.
+
+hoare addstate_array_avx2_h _st _buf _off _len _tb:
+ M(P).__addstate_array_avx2
+ : st=_st /\ buf=_buf /\ offset=_off /\ lEN=_len /\ tRAILB=_tb
+   /\ 0 <= _len <= 200 - b2i (_tb<>0)
+   /\ to_uint offset + _len <= aSIZE
+ ==> let l = sub _buf (to_uint _off) _len ++ if _tb <> 0 then [W8.of_int _tb] else []
+     in res.`1 = addstavx2 _st l
+     /\ res.`2 = _off + (W64.of_int _len).
+proof.
+proc.
+admit.
+qed.
+
+(*
+absorb_array_avx2
+*)
+lemma absorb_array_avx2_ll: islossless M(P).__absorb_array_avx2.
+proof.
+proc*.
+admit.
+qed.
+
+hoare absorb_array_avx2_h _st _buf _off _len _r8 _tb:
+ M(P).__absorb_array_avx2
+ : st=_st /\ buf=_buf /\ offset=_off /\ lEN=_len /\ rATE8=_r8 /\ tRAILB=_tb
+ ==> res.`1 = stavx2_from_st25 (ABSORB1600 (W8.of_int _tb) _r8 (sub _buf (to_uint _off) _len))
+  /\ res.`2 = _off + W64.of_int _len.
+proof.
+admit.
+qed.
+
+phoare absorb_array_avx2_ph _st _buf _off _len _r8 _tb:
+ [ M(P).__absorb_array_avx2
+ : st=_st /\ buf=_buf /\ offset=_off /\ lEN=_len /\ rATE8=_r8 /\ tRAILB=_tb
+ ==> res.`1 = stavx2_from_st25 (ABSORB1600 (W8.of_int _tb) _r8 (sub _buf (to_uint _off) _len))
+  /\ res.`2 = _off + W64.of_int _len
+ ] = 1%r.
+proof.
+by conseq absorb_array_avx2_ll (absorb_array_avx2_h _st _buf _off _len _r8 _tb).
+qed.
+
+
+(*
+   INCREMENTAL (FIXED-SIZE) MEMORY ABSORB
+   ======================================
+*)
+
+op fillpst_at (st: W64.t Array25.t) (at:int) (l: W8.t list) =
+ stwords
+  (WArray200.fill 
+   (fun i => nth W8.zero l (i-at)) at (size l) (stbytes st)).
+
+(*
+pstate_array_avx2
+*)
+lemma pstate_array_avx2_ll: islossless M(P).__pstate_array_avx2.
+proc.
+print stwords.
+admitted.
+
+hoare pstate_array_avx2_h _pst _at _buf _off _len _tb:
+ M(P).__pstate_array_avx2
+ : pst=_pst /\ aT=_at /\ buf=_buf /\ offset=_off /\ lEN=_len /\ tRAILB=_tb
+ /\ 0 <= _at <= _at + _len <= 200 - b2i (_tb<>0)
+ /\ to_uint _off + _len <= aSIZE
+ ==> let l = sub _buf (to_uint _off) _len ++ if _tb <> 0 then [W8.of_int _tb] else []
+     in res.`1 = fillpst_at _pst _at l
+     /\ res.`2 = _at + size l
+     /\ res.`3 = _off + (W64.of_int _len).
+admitted.
+
+phoare pstate_array_avx2_ph _pst _at _buf _off _len _tb:
+ [ M(P).__pstate_array_avx2
+ : pst=_pst /\ aT=_at /\ buf=_buf /\ offset=_off /\ lEN=_len /\ tRAILB=_tb
+ /\ 0 <= _at <= _at + _len <= 200 - b2i (_tb<>0)
+ /\ to_uint _off + _len <= aSIZE
+ ==> let l = sub _buf (to_uint _off) _len ++ if _tb <> 0 then [W8.of_int _tb] else []
+     in res.`1 = fillpst_at _pst _at l
+     /\ res.`2 = _at + size l
+     /\ res.`3 = _off + (W64.of_int _len)
+ ] = 1%r.
+proof.
+by conseq pstate_array_avx2_ll (pstate_array_avx2_h _pst _at _buf _off _len _tb).
+qed.
+
+(*
+pabsorb_array_avx2
+*)
+lemma pabsorb_array_avx2_ll: islossless M(P).__pabsorb_array_avx2.
+admitted.
+
+op addst_at (st: W64.t Array25.t) at l =
+ let st200 = stbytes st in
+ stwords
+  (WArray200.fill 
+   (fun i => st200.[i] `^` (nth W8.zero l (i-at))) at (size l) st200).
+
+require BitEncoding.
+import BitEncoding.BitChunking.
+
+print chunkremains.
+print ABSORB1600.
+print stateabsorb_last.
+print state2bytes.
+print stateabsorb_iblocks.
+op pabsorb_update_spec_avx2 (r8: int, pst: W64.t Array25.t, st: W256.t Array7.t, l: W8.t list): bool =
+ let st' = stavx2_from_st25 (stateabsorb_iblocks (chunk r8 l) st0)
+ in let l' = chunkremains r8 l
+ in st=st' /\
+    take (size l'+1) (state2bytes pst)=l'.
+print ABSORB1600.
+
+op absorb_spec_avx2 (r8: int) (tb: int) (st: W256.t Array7.t) (l: W8.t list) =
+ st = stavx2_from_st25 (ABSORB1600 (W8.of_int tb) r8 l).
+
+
+op pabsorb_spec_avx2 (r8: int) st0 l' (st: W256.t Array7.t) (l: W8.t list): bool =
+ 0 < r8 <= 200 /\
+ st=stavx2_from_st25 (stateabsorb_iblocks (chunk r8 l) (stavx2_to_st25 st0)) /\
+ l' = chunkremains r8 l.
+
+lemma pabsorb_spec_avx2_nil r8:
+ 0 < r8 <= 200 =>
+ pabsorb_spec_avx2 r8 (stavx2_from_st25 st0) [] (stavx2_from_st25 st0) [].
+proof.
+move=> Hr; rewrite /pabsorb_spec_avx2 => />.
+rewrite chunk0 /= 1:/#.
+rewrite stavx2_from_st25K.
+by rewrite /stateabsorb_iblocks /= /chunkremains.
+qed.
+
+lemma pabsorb_spec_avx2_cat r8 st0 l1 st1 l12 l2 st2 l22:
+ pabsorb_spec_avx2 r8 st0 l12 st1 l1 =>
+ pabsorb_spec_avx2 r8 st1 l22 st2 (l12++l2)=>
+ pabsorb_spec_avx2 r8 st0 l22 st2 (l1++l2).
+proof.
+rewrite /pabsorb_spec_avx2 => /> Hr0 Hr1; split.
+ admit.
+admit.
+qed.
+
+hoare pabsorb_array_avx2_h _l _buf _off _len _r8 _tb:
+ M(P).__pabsorb_array_avx2
+ : buf=_buf /\ offset=_off /\ lEN=_len /\ rATE8=_r8 /\ tRAILB=_tb
+ /\ aT = size _l %% _r8
+ /\ pabsorb_spec_avx2 _r8 (stavx2_from_st25 st0) (sub (stbytes pst) 0 aT) st _l
+ ==> if _tb <> 0
+     then absorb_spec_avx2 _r8 _tb res.`3 (_l ++ sub _buf (to_uint _off) _len)
+     else pabsorb_spec_avx2 _r8 (stavx2_from_st25 st0) (sub (stbytes res.`1) 0 res.`2) res.`3 (_l ++ sub _buf (to_uint _off) _len)
+          /\ res.`2 = (size _l + _len) %% _r8
+          /\ res.`4 = _off + W64.of_int _len.
+admitted.
+(* ==> let l = sub _buf (to_uint _off) _len ++ if _tb <> 0 then [W8.of_int _tb] else []
+     in res.`1 = fillpst_at _pst _at l
+     /\ res.`2 = _at + size l
+     /\ res.`3 = 
+     /\ res.`3 = _off + (W64.of_int _len).*)
+
+(*
+hoare pabsorb_array_avx2_h _pst _at _st _buf _off _len _r8 _tb:
+ M(P).__pabsorb_array_avx2
+ : pst=_pst /\ aT=_at /\ st=_st /\ buf=_buf /\ offset=_off /\ lEN=_len /\ rATE8=_r8 /\ tRAILB=_tb
+ /\ 0 <= _at < 200
+ /\ to_uint _off + _len <= aSIZE
+(* ==> let l = sub _buf (to_uint _off) _len ++ if _tb <> 0 then [W8.of_int _tb] else []
+     in res.`1 = fillpst_at _pst _at l
+     /\ res.`2 = _at + size l
+     /\ res.`3 = 
+     /\ res.`3 = _off + (W64.of_int _len).*)
+ ==> res=res.
+proc.
+admitted.
+*)
+
+
+(*
+   ONE-SHOT (FIXED-SIZE) MEMORY SQUEEZE
+   ====================================
+*)
+
+(*
+dumpstate_array_avx2
+*)
+lemma dumpstate_array_avx2_ll: islossless M(P).__dumpstate_array_avx2
+ by islossless.
+
+hoare dumpstate_array_avx2_h _buf _off _len _st:
+ M(P).__dumpstate_array_avx2
+ : buf=_buf /\ offset=_off /\ lEN=_len /\ st=_st
+ ==> true.
+admitted.
+
+(*
+squeeze_array_avx2
+*)
+lemma squeeze_array_avx2_ll: islossless M(P).__squeeze_array_avx2.
+admitted.
+
+hoare squeeze_array_avx2_h _buf _off _len _st _r8:
+ M(P).__squeeze_array_avx2
+ : buf=_buf /\ offset=_off /\ lEN=_len /\ st=_st /\ rATE8=_r8
+ ==> true.
+admitted.
