proof/amd64/avx2/Keccak1600_imem_avx2.ec
@@ -1,0 +1,118 @@
+(******************************************************************************
+   Keccak1600_imem_avx2.ec:
+
+   Correctness proof for the Keccak (fixed-sized) memory absorb/squeeze
+  AVX2 implementation
+
+
+
+******************************************************************************)
+
+require import List Real Distr Int IntDiv CoreMap.
+
+from Jasmin require import JModel.
+
+from CryptoSpecs require export Keccakf1600_Spec.
+
+require import WArray768.
+from JazzEC require import Jazz_avx2.
+
+require import Array4 Array5 Array7 Array24 Array25.
+
+from CryptoSpecs require import FIPS202_Keccakf1600.
+from CryptoSpecs require import Keccakf1600_Spec.
+
+
+(*
+   ONE-SHOT (FIXED-SIZE) MEMORY ABSORB
+   ===================================
+*)
+
+(*
+addstate_imem_avx2
+*)
+lemma addstate_imem_avx2_ll: islossless M.__addstate_imem_avx2
+ by islossless.
+
+hoare addstate_imem_avx2_h _st _buf _len _trailb:
+ M.__addstate_imem_avx2
+ : st=_st /\ buf=_buf /\ lEN=_len /\ tRAILB=_trailb
+ ==> true.
+proof.
+admit.
+qed.
+
+(*
+absorb_imem_avx2
+*)
+lemma absorb_imem_avx2_ll: islossless M.__absorb_imem_avx2.
+proof.
+proc*.
+admit.
+qed.
+
+hoare absorb_imem_avx2_h _st _buf _len _r8 _trailb:
+ M.__absorb_imem_avx2
+ : st=_st /\ buf=_buf /\ lEN=_len /\ rATE8=_r8 /\ tRAILB=_trailb
+ ==> true.
+admit.
+qed.
+
+
+(*
+   INCREMENTAL (FIXED-SIZE) MEMORY ABSORB
+   ======================================
+*)
+
+(*
+pstate_imem_avx2
+*)
+lemma pstate_imem_avx2_ll: islossless M.__pstate_imem_avx2.
+admitted.
+
+hoare pstate_imem_avx2_h _pst _at _buf _len _trailb:
+ M.__pstate_imem_avx2
+ : pst=_pst /\ aT=_at /\ buf=_buf /\ lEN=_len /\ tRAILB=_trailb
+ ==> true.
+admitted.
+
+(*
+pabsorb_imem_avx2
+*)
+lemma pabsorb_imem_avx2_ll: islossless M.__pabsorb_imem_avx2.
+admitted.
+
+hoare pabsorb_imem_avx2_h _pst _at _st _buf _len _r8 _trailb:
+ M.__pabsorb_imem_avx2
+ : pst=_pst /\ aT=_at /\ st=_st /\ buf=_buf /\ lEN=_len /\ rATE8=_r8 /\ tRAILB=_trailb
+ ==> true.
+admitted.
+
+(*
+   ONE-SHOT (FIXED-SIZE) MEMORY SQUEEZE
+   ====================================
+*)
+
+(*
+dumpstate_imem_avx2
+*)
+lemma dumpstate_imem_avx2_ll: islossless M.__dumpstate_imem_avx2
+ by islossless.
+
+hoare dumpstate_imem_avx2_h _buf _len _st:
+ M.__dumpstate_imem_avx2
+ : buf=_buf /\ lEN=_len /\ st=_st
+ ==> true.
+admitted.
+
+(*
+squeeze_imem_avx2
+*)
+lemma squeeze_imem_avx2_ll: islossless M.__squeeze_imem_avx2.
+admitted.
+
+hoare squeeze_imem_avx2_h _buf _len _st _r8:
+ M.__squeeze_imem_avx2
+ : buf=_buf /\ lEN=_len /\ st=_st /\ rATE8=_r8
+ ==> true.
+admitted.
