proof/amd64/ref/Keccakf1600_ref.ec
@@ -1,0 +1,278 @@
+(******************************************************************************
+   Keccakf1600_ref.ec:
+
+   Correctness proof for the Keccak REF implementation
+******************************************************************************)
+require import List Real Int IntDiv CoreMap.
+
+from Jasmin require import JModel.
+(*
+require import Keccak_f1600_Spec_facts.
+require import Keccak_f1600_s_spec_proof.
+*)
+
+from CryptoSpecs require import FIPS202_Keccakf1600.
+from CryptoSpecs require import Keccakf1600_Spec.
+from CryptoSpecs require import Bindings.
+
+from JazzEC require import Jazz_ref.
+from JazzEC require import Array5 Array24.
+
+(** lemmata (move?) *)
+
+lemma ROL_64_by0 (w: W64.t): w `|<<<|` 0 = w.
+proof. by apply  W64.all_eq_eq; rewrite /all_eq /=. qed.
+
+lemma ROL_64_val w i:
+ (ROL_64 w (W8.of_int i)).`3 = w `|<<<|` (i %% 64).
+proof.
+rewrite /ROL_64 /shift_mask /=.
+rewrite modz_dvd 1:/#.
+case: (i %% 64 = 0) => [->|//].
+by apply W64.all_eq_eq; rewrite /all_eq.
+qed.
+
+hoare rol_u64_h _x _r:
+ M.__rol_u64_ref
+ : x = _x /\ i = _r%%64
+ ==> res = _x  `|<<<|` _r%%64.
+proof.
+proc; simplify.
+case: (i=0).
+ by rcondf 1; auto => /> ->; rewrite ROL_64_by0.
+rcondt 1; auto => /> E.
+rewrite /ROL_64 /shift_mask /=.
+by rewrite !modz_dvd 1..2:/# E.
+qed.
+
+lemma rol_u64_ll: islossless M.__rol_u64_ref
+ by islossless.
+
+phoare rol_u64_ph _x _r:
+ [ M.__rol_u64_ref
+ : x = _x /\ i = _r%%64 ==> res = _x  `|<<<|` _r%%64 ] = 1%r
+by conseq rol_u64_ll (rol_u64_h _x _r).
+
+
+(* *)
+
+hoare theta_sum_ref_h _a:
+ M.__theta_sum_ref :
+  a = _a ==> res = keccak_C _a.
+proof.
+proc.
+do 6! unroll for ^while.
+auto => />.
+by rewrite -Array5.ext_eq_all /all_eq /keccak_C /idx /invidx /=.
+qed.
+
+hoare theta_rol_ref_h _c:
+ M.__theta_rol_ref :
+  c = _c ==> res = keccak_D _c.
+proof.
+proc.
+unroll for ^while; inline*; auto => />.
+rewrite -ext_eq_all /all_eq /keccak_D /idx /invidx /=.
+by rewrite /ROL_64 /shift_mask /init_5_64 /rol_64 /=; smt(W64.xorwC).
+qed.
+
+hoare keccak_rho_offsets_h _i:
+  M.keccakf1600_rho_offsets:
+  0 <= i < 25 /\ i = _i ==> res = to_uint rhotates.[_i].
+proof.
+proc.
+while (0 <= t <= 24 /\ i=_i /\ 0 <= x < 5 /\ 0 <= y < 5 /\
+       (x,y,r) = foldl (fun (a:_*_*_) t =>
+                           ( a.`2
+                           , (2*a.`1+3*a.`2)%%5
+                           , if i=idx(a.`1,a.`2) then (t+1)*(t+2) %/ 2 %% 64 else a.`3)) 
+                       (1,0,0) (iota_ 0 t)).
+ auto => &m [[Ht [Hi [Hx [Hy IH]]]] Hc]; split.
+  move=> P /=; split; first smt().
+  by rewrite iotaSr 1:/# foldl_rcons /= -IH /= /#. 
+ move=> P /=; split; first smt().
+ by rewrite iotaSr 1:/# foldl_rcons /= -IH /= /#. 
+auto => /> Hi0 Hi1; split.
+ by rewrite -iotaredE /=.
+move=> r t x y ???; have ->: t=24 by smt().
+move => _ _ _ _.
+have: _i \in iota_ 0 25 by smt(mem_iota).
+move: {Hi0 Hi1} _i; apply/List.allP.
+by rewrite -iotaredE /rhotates /= /#.
+qed.
+
+lemma rhotates_idx_mod64 _i:
+ 0 <= _i < 25 =>
+ to_uint rhotates.[_i] %% 64 = to_uint rhotates.[_i].
+proof.
+move=> Hi; have: _i \in iota_ 0 25.
+ by rewrite mem_iota; smt(idx_bnd).
+by move: {Hi} _i ; rewrite -allP -iotaredE /= initiE /=.
+qed.
+
+hoare rhotates_spec_h _x _y:
+  M.keccakf1600_rhotates :
+  x = _x /\ y = _y /\ 0<=_x<5 /\ 0<=_y<5 ==> res = to_uint rhotates.[idx(_x,_y)].
+proof.
+proc.
+call (keccak_rho_offsets_h (idx(_x,_y))).
+by inline*; auto => /> * /#.
+qed.
+
+hoare rol_sum_ref_h _a _y:
+ M.__rol_sum_ref :
+  a = _a /\ d = keccak_D (keccak_C _a) /\ y = _y /\ 0 <= y < 5
+  ==> forall x, 0 <= x < 5 => res.[x] = (keccak_pi_op (keccak_rho_op (keccak_theta_op _a))).[idx(x,_y)].
+proof.
+proc; simplify.
+while (#pre /\ 0 <= x <= 5 /\
+       forall i, 0 <= i < x =>
+        b.[i] =
+        rol_64 (_a.[idx (i + 3 * _y, i)] 
+                `^` (keccak_D (keccak_C _a)).[(i+3*_y)%%5])
+        (rhotates.[idx (i + 3 * _y, i)])).
+ wp; ecall (rol_u64_h b.[x] r).
+ wp; ecall (rhotates_spec_h x_ y_).
+ auto => /> &m Hy1 Hy2 Hx1 _ IH Hx2; split; first smt().
+ move=> Hz1 Hz2; split.
+  by rewrite rhotates_idx_mod64 /#.
+ move => _; split; first by smt().
+ move => i Hi1 Hi2.
+ case: (i = x{m}) => E.
+  rewrite E get_setE 1:/# ifT 1:/#.
+  rewrite get_setE 1:/# ifT 1:/#.
+  rewrite get_setE 1:/# ifT 1:/#.
+  by rewrite rhotates_idx_mod64 /rol_64 1:/# modz_mod /idx_op /#.
+ by rewrite get_setE 1:/# ifF 1:/# IH 1:/#.
+auto => /> Hy1 Hy2; split; first by smt().
+move => A k ???; have ->:k=5 by smt().
+move => IH x Hx1 Hx2.
+rewrite IH 1:/#.
+pose R:= rhotates.[_] (*obs: lock reduction *).
+rewrite /rol_64 /init_25_64 /=.
+rewrite Array25.initiE 1:/#; beta. 
+rewrite -/(idx_op (x,_y)) -/(invidx_op _) idxK' /idx_op /=.
+rewrite Array25.initiE 1:/# //= /rol_64 !modz_mod.
+rewrite Array25.initiE 1:/# //= /rol_64; congr; congr; smt(). 
+qed.
+
+hoare ANDN_64_h _a _b:
+ M.__ANDN_64 :
+ a = _a /\ b = _b ==> res = invw _a `&` _b.
+proof. by proc; auto. qed.
+
+phoare ANDN_64_ph _a _b:
+ [ M.__ANDN_64 :
+   a = _a /\ b = _b ==> res = invw _a `&` _b ] = 1%r.
+proof. by proc; auto. qed.
+
+hoare set_row_ref_h _a _e _b _y _c:
+ M.__set_row_ref :
+  e = _e /\ b = _b /\ y = _y /\ s_rc = _c /\ 0 <= y < 5
+  /\ (forall x, 0 <= x < 5 =>
+      _b.[x] = (keccak_pi_op (keccak_rho_op (keccak_theta_op _a))).[idx(x,_y)])
+  /\ (forall k, 0 <= k < 5*_y => e.[k] = (keccak_round_op _c _a).[k])
+  ==> forall k, 0 <= k < 5*_y + 5 => res.[k] = (keccak_round_op _c _a).[k].
+proof.
+proc; simplify.
+while (#[/2:7]pre /\ 0 <= x <= 5 /\ 
+       forall k, 0 <= k < x+5*_y => e.[k] = (keccak_round_op _c _a).[k]).
+ wp; ecall (ANDN_64_h b.[x1] b.[x2]).
+ auto => /> &m Hy1 Hy2 Hb Hx1 _ IH Hx2; split.
+  move => Ex Ey k ??; have ->: k=0 by smt().
+  rewrite get_setE 1:/# ifT 1:/#.
+  rewrite /keccak_round_op /keccak_iota_op /keccak_chi_op /=.
+  rewrite !Hb // /invidx /idx Ey /=.
+  by congr; rewrite W64.xorwC.
+ move => E0; split; first smt().
+ move=> k Hk1 Hk2.
+ case: (k = x{m}+5*_y) => E.
+  rewrite /keccak_round_op /keccak_iota_op /keccak_chi_op /=.
+  rewrite eq_sym get_setE 1:/# ifF 1:/#.
+  rewrite get_setE 1:/# ifT 1:/#.
+  rewrite !Hb 1..3:/# /=.
+  rewrite initiE 1:/# E /= xorwC; congr; congr; smt().
+ by rewrite get_setE 1:/# ifF 1:/# -IH /#.
+by auto => /> Hy1 Hy2 _ H e k ???; have ->: k=5; smt().
+qed.
+
+hoare round_ref_h _a _c:
+ M.__round_ref :
+  a = _a /\ s_rc = _c ==> res = keccak_round_op _c _a.
+proof.
+proc; simplify.
+while (0 <= y <= 5 /\ #pre /\
+       d = keccak_D (keccak_C _a) /\
+       forall k, 0 <= k < 5*y => 
+        e.[k] = (keccak_round_op _c _a).[k]).
+ wp; ecall (set_row_ref_h a e b y s_rc).
+ simplify; ecall (rol_sum_ref_h a y); simplify.
+ auto => /> &m Hy1 _ IH Hy2 b Hb e He; split; smt().
+wp; ecall (theta_rol_ref_h c).
+ecall (theta_sum_ref_h a).
+auto => /> &m; split; first smt().
+move=> e y ???; have ->: y=5 by smt().
+by move=> /= H; apply Array25.ext_eq => k Hk; apply H.
+qed.
+
+lemma round_ref_ll: islossless M.__round_ref.
+proof.
+proc; inline*.
+do 43! unroll for ^while.
+by islossless.
+qed.
+
+require import List.
+import BitEncoding.BitChunking.
+
+abbrev keccak_double_round A i =
+ keccak_round_op rc_spec.[2*i+1] (keccak_round_op rc_spec.[2*i] A).
+
+hoare keccakf1600_ref_h _a:
+ M.__keccakf1600_ref :
+  a = _a ==> res = keccak_f1600_op _a.
+proof.
+proc.
+while (2 <= to_uint c <= 24 /\ 2 %| to_uint c /\
+       s_RC = kECCAK1600_RC /\
+       keccak_f1600_op _a = foldl keccak_double_round a (range (to_uint c %/ 2) 12)).
+ wp; ecall (round_ref_h e s_rc).
+ wp; ecall (round_ref_h a s_rc).
+ auto => /> &m Hc1 _ Hc_2 IH.
+ rewrite ultE of_uintK /= => Hc2; split.
+  by rewrite to_uintD_small /#.
+ rewrite to_uintD_small 1:/#.
+ move: IH; rewrite (range_cat (to_uint c{m} %/ 2 + 1)) 1..2:/#.
+ by rewrite /rc_spec rangeS foldl_cat /= => -> /#.
+wp; ecall (round_ref_h e s_rc).
+wp; ecall (round_ref_h a s_rc).
+auto => />; split.
+ by rewrite /keccak_f1600_op /range /rc_spec -iotaredE.
+move => a c; rewrite ultE /= => ????.
+have ->/=: to_uint c = 24 by smt().
+by rewrite range_geq /=.
+qed.
+
+lemma keccakf1600_ref_ll: islossless M.__keccakf1600_ref.
+proc.
+have Hll:= round_ref_ll.
+wp; while (0 <= to_uint c <= 24) (23 - to_uint c).
+ move=> z.
+ wp; call round_ref_ll.
+ wp; call round_ref_ll.
+ auto => /> &m ?_.
+ rewrite ultE of_uintK /= => ?.
+ by rewrite to_uintD_small of_uintK /= /#.
+wp; call round_ref_ll.
+wp; call round_ref_ll.
+auto => /> c ???.
+by rewrite ultE of_uintK /= /#.
+qed.
+
+phoare keccakf1600_ref_ph _a:
+ [ M.__keccakf1600_ref
+ : a = _a
+ ==> res = keccak_f1600_op _a
+ ] = 1%r.
+proof. by conseq keccakf1600_ref_ll (keccakf1600_ref_h _a). qed.
+
