proof/extracted/Jazz_ref.ec
@@ -1,0 +1,668 @@
+require import AllCore IntDiv CoreMap List Distr.
+
+from Jasmin require import JModel_x86.
+
+import SLH64.
+
+require import Array5 Array24 Array25 WArray40 WArray192 WArray200.
+
+abbrev kECCAK1600_RC =
+(Array24.of_list witness
+[(W64.of_int 1); (W64.of_int 32898); (W64.of_int (-9223372036854742902));
+(W64.of_int (-9223372034707259392)); (W64.of_int 32907);
+(W64.of_int 2147483649); (W64.of_int (-9223372034707259263));
+(W64.of_int (-9223372036854743031)); (W64.of_int 138); (W64.of_int 136);
+(W64.of_int 2147516425); (W64.of_int 2147483658); (W64.of_int 2147516555);
+(W64.of_int (-9223372036854775669)); (W64.of_int (-9223372036854742903));
+(W64.of_int (-9223372036854743037)); (W64.of_int (-9223372036854743038));
+(W64.of_int (-9223372036854775680)); (W64.of_int 32778);
+(W64.of_int (-9223372034707292150)); (W64.of_int (-9223372034707259263));
+(W64.of_int (-9223372036854742912)); (W64.of_int 2147483649);
+(W64.of_int (-9223372034707259384))]).
+
+module M = {
+  proc __ANDN_64 (a:W64.t, b:W64.t) : W64.t = {
+    var t:W64.t;
+    t <- a;
+    t <- (invw t);
+    t <- (t `&` b);
+    return t;
+  }
+  proc keccakf1600_index (x:int, y:int) : int = {
+    var r:int;
+    r <- ((x %% 5) + (5 * (y %% 5)));
+    return r;
+  }
+  proc keccakf1600_rho_offsets (i:int) : int = {
+    var aux:int;
+    var r:int;
+    var x:int;
+    var y:int;
+    var t:int;
+    var z:int;
+    r <- 0;
+    x <- 1;
+    y <- 0;
+    t <- 0;
+    while ((t < 24)) {
+      if ((i = (x + (5 * y)))) {
+        r <- ((((t + 1) * (t + 2)) %/ 2) %% 64);
+      } else {
+        
+      }
+      z <- (((2 * x) + (3 * y)) %% 5);
+      x <- y;
+      y <- z;
+      t <- (t + 1);
+    }
+    return r;
+  }
+  proc keccakf1600_rhotates (x:int, y:int) : int = {
+    var r:int;
+    var i:int;
+    i <@ keccakf1600_index (x, y);
+    r <@ keccakf1600_rho_offsets (i);
+    return r;
+  }
+  proc __rol_u64_ref (x:W64.t, i:int) : W64.t = {
+    var  _0:bool;
+    var  _1:bool;
+    if ((i <> 0)) {
+      ( _0,  _1, x) <- (ROL_64 x (W8.of_int i));
+    } else {
+      
+    }
+    return x;
+  }
+  proc __theta_sum_ref (a:W64.t Array25.t) : W64.t Array5.t = {
+    var aux:int;
+    var c:W64.t Array5.t;
+    var x:int;
+    var y:int;
+    c <- witness;
+    x <- 0;
+    while ((x < 5)) {
+      c.[x] <- a.[(x + 0)];
+      x <- (x + 1);
+    }
+    y <- 1;
+    while ((y < 5)) {
+      x <- 0;
+      while ((x < 5)) {
+        c.[x] <- (c.[x] `^` a.[(x + (y * 5))]);
+        x <- (x + 1);
+      }
+      y <- (y + 1);
+    }
+    return c;
+  }
+  proc __theta_rol_ref (c:W64.t Array5.t) : W64.t Array5.t = {
+    var aux:int;
+    var aux_0:W64.t;
+    var d:W64.t Array5.t;
+    var x:int;
+    d <- witness;
+    x <- 0;
+    while ((x < 5)) {
+      d.[x] <- c.[((x + 1) %% 5)];
+      aux_0 <@ __rol_u64_ref (d.[x], 1);
+      d.[x] <- aux_0;
+      d.[x] <- (d.[x] `^` c.[(((x - 1) + 5) %% 5)]);
+      x <- (x + 1);
+    }
+    return d;
+  }
+  proc __rol_sum_ref (a:W64.t Array25.t, d:W64.t Array5.t, y:int) : W64.t Array5.t = {
+    var aux:int;
+    var aux_0:W64.t;
+    var b:W64.t Array5.t;
+    var x:int;
+    var x_:int;
+    var y_:int;
+    var r:int;
+    b <- witness;
+    x <- 0;
+    while ((x < 5)) {
+      x_ <- ((x + (3 * y)) %% 5);
+      y_ <- x;
+      r <@ keccakf1600_rhotates (x_, y_);
+      b.[x] <- a.[(x_ + (y_ * 5))];
+      b.[x] <- (b.[x] `^` d.[x_]);
+      aux_0 <@ __rol_u64_ref (b.[x], r);
+      b.[x] <- aux_0;
+      x <- (x + 1);
+    }
+    return b;
+  }
+  proc __set_row_ref (e:W64.t Array25.t, b:W64.t Array5.t, y:int, s_rc:W64.t) : 
+  W64.t Array25.t = {
+    var aux:int;
+    var x:int;
+    var x1:int;
+    var x2:int;
+    var t:W64.t;
+    x <- 0;
+    while ((x < 5)) {
+      x1 <- ((x + 1) %% 5);
+      x2 <- ((x + 2) %% 5);
+      t <@ __ANDN_64 (b.[x1], b.[x2]);
+      t <- (t `^` b.[x]);
+      if (((x = 0) /\ (y = 0))) {
+        t <- (t `^` s_rc);
+      } else {
+        
+      }
+      e.[(x + (y * 5))] <- t;
+      x <- (x + 1);
+    }
+    return e;
+  }
+  proc __round_ref (e:W64.t Array25.t, a:W64.t Array25.t, s_rc:W64.t) : 
+  W64.t Array25.t = {
+    var aux:int;
+    var c:W64.t Array5.t;
+    var d:W64.t Array5.t;
+    var y:int;
+    var b:W64.t Array5.t;
+    b <- witness;
+    c <- witness;
+    d <- witness;
+    c <@ __theta_sum_ref (a);
+    d <@ __theta_rol_ref (c);
+    y <- 0;
+    while ((y < 5)) {
+      b <@ __rol_sum_ref (a, d, y);
+      e <@ __set_row_ref (e, b, y, s_rc);
+      y <- (y + 1);
+    }
+    return e;
+  }
+  proc __keccakf1600_ref (a:W64.t Array25.t) : W64.t Array25.t = {
+    var rC:W64.t Array24.t;
+    var s_RC:W64.t Array24.t;
+    var s_e:W64.t Array25.t;
+    var e:W64.t Array25.t;
+    var c:W64.t;
+    var s_c:W64.t;
+    var rc:W64.t;
+    var s_rc:W64.t;
+    rC <- witness;
+    e <- witness;
+    s_RC <- witness;
+    s_e <- witness;
+    rC <- kECCAK1600_RC;
+    s_RC <- rC;
+    e <- s_e;
+    c <- (W64.of_int 0);
+    s_c <- c;
+    rC <- s_RC;
+    rc <- rC.[(W64.to_uint c)];
+    s_rc <- rc;
+    e <@ __round_ref (e, a, s_rc);
+    rC <- s_RC;
+    rc <- rC.[((W64.to_uint c) + 1)];
+    s_rc <- rc;
+    a <@ __round_ref (a, e, s_rc);
+    c <- s_c;
+    c <- (c + (W64.of_int 2));
+    while ((c \ult (W64.of_int (24 - 1)))) {
+      s_c <- c;
+      rC <- s_RC;
+      rc <- rC.[(W64.to_uint c)];
+      s_rc <- rc;
+      e <@ __round_ref (e, a, s_rc);
+      rC <- s_RC;
+      rc <- rC.[((W64.to_uint c) + 1)];
+      s_rc <- rc;
+      a <@ __round_ref (a, e, s_rc);
+      c <- s_c;
+      c <- (c + (W64.of_int 2));
+    }
+    return a;
+  }
+  proc _keccakf1600_ref (a:W64.t Array25.t) : W64.t Array25.t = {
+    
+    a <@ __keccakf1600_ref (a);
+    return a;
+  }
+  proc _keccakf1600_ref_ (a:W64.t Array25.t) : W64.t Array25.t = {
+    
+    a <- a;
+    a <@ _keccakf1600_ref (a);
+    a <- a;
+    return a;
+  }
+  proc __state_init_ref (st:W64.t Array25.t) : W64.t Array25.t = {
+    var z64:W64.t;
+    var i:W64.t;
+    z64 <- (W64.of_int 0);
+    i <- (W64.of_int 0);
+    while ((i \ult (W64.of_int 25))) {
+      st.[(W64.to_uint i)] <- z64;
+      i <- (i + (W64.of_int 1));
+    }
+    return st;
+  }
+  proc __addratebit_ref (st:W64.t Array25.t, rATE8:int) : W64.t Array25.t = {
+    var t64:W64.t;
+    t64 <- (W64.of_int 1);
+    t64 <- (t64 `<<` (W8.of_int (((8 * rATE8) - 1) %% 64)));
+    t64 <- (t64 `^` st.[((rATE8 - 1) %/ 8)]);
+    st.[((rATE8 - 1) %/ 8)] <- t64;
+    return st;
+  }
+  proc __mread_subu64 (buf:W64.t, lEN:int, tRAIL:int) : W64.t * int * int *
+                                                        W64.t = {
+    var w:W64.t;
+    var iLEN:int;
+    var t16:W64.t;
+    var t8:W64.t;
+    iLEN <- lEN;
+    if ((lEN <= 0)) {
+      w <- (W64.of_int tRAIL);
+      tRAIL <- 0;
+    } else {
+      if ((8 <= lEN)) {
+        w <- (loadW64 Glob.mem (W64.to_uint (buf + (W64.of_int 0))));
+        buf <- (buf + (W64.of_int 8));
+        lEN <- (lEN - 8);
+      } else {
+        if ((4 <= lEN)) {
+          w <-
+          (zeroextu64 (loadW32 Glob.mem (W64.to_uint (buf + (W64.of_int 0))))
+          );
+          buf <- (buf + (W64.of_int 4));
+          lEN <- (lEN - 4);
+        } else {
+          w <- (W64.of_int 0);
+        }
+        if ((2 <= lEN)) {
+          t16 <-
+          (zeroextu64 (loadW16 Glob.mem (W64.to_uint (buf + (W64.of_int 0))))
+          );
+          buf <- (buf + (W64.of_int 2));
+          lEN <- (lEN - 2);
+        } else {
+          t16 <- (W64.of_int 0);
+        }
+        if (((1 <= lEN) \/ (tRAIL <> 0))) {
+          if ((1 <= lEN)) {
+            t8 <-
+            (zeroextu64
+            (loadW8 Glob.mem (W64.to_uint (buf + (W64.of_int 0)))));
+            if ((tRAIL <> 0)) {
+              t8 <- (t8 `|` (W64.of_int (256 * tRAIL)));
+            } else {
+              
+            }
+            buf <- (buf + (W64.of_int 1));
+            lEN <- (lEN - 1);
+          } else {
+            t8 <- (W64.of_int tRAIL);
+          }
+          tRAIL <- 0;
+          t8 <- (t8 `<<` (W8.of_int (8 * (2 * ((iLEN %/ 2) %% 2)))));
+          t16 <- (t16 `|` t8);
+        } else {
+          
+        }
+        t16 <- (t16 `<<` (W8.of_int (8 * (4 * ((iLEN %/ 4) %% 2)))));
+        w <- (w `|` t16);
+      }
+    }
+    return (buf, lEN, tRAIL, w);
+  }
+  proc __mread_bcast_4subu64 (buf:W64.t, lEN:int, tRAIL:int) : W64.t * int *
+                                                               int * W256.t = {
+    var w:W256.t;
+    var t64:W64.t;
+    var t128:W128.t;
+    if (((lEN <= 0) /\ (tRAIL = 0))) {
+      w <- (set0_256);
+    } else {
+      if ((8 <= lEN)) {
+        w <-
+        (VPBROADCAST_4u64
+        (loadW64 Glob.mem (W64.to_uint (buf + (W64.of_int 0)))));
+        buf <- (buf + (W64.of_int 8));
+        lEN <- (lEN - 8);
+      } else {
+        (buf, lEN, tRAIL, t64) <@ __mread_subu64 (buf, lEN, tRAIL);
+        t128 <- (zeroextu128 t64);
+        w <- (VPBROADCAST_4u64 (truncateu64 t128));
+      }
+    }
+    return (buf, lEN, tRAIL, w);
+  }
+  proc __mread_subu128 (buf:W64.t, lEN:int, tRAIL:int) : W64.t * int * int *
+                                                         W128.t = {
+    var w:W128.t;
+    var t64:W64.t;
+    if (((lEN <= 0) /\ (tRAIL = 0))) {
+      w <- (set0_128);
+    } else {
+      if ((16 <= lEN)) {
+        w <- (loadW128 Glob.mem (W64.to_uint (buf + (W64.of_int 0))));
+        buf <- (buf + (W64.of_int 16));
+        lEN <- (lEN - 16);
+      } else {
+        if ((8 <= lEN)) {
+          w <-
+          (VMOV_64 (loadW64 Glob.mem (W64.to_uint (buf + (W64.of_int 0)))));
+          buf <- (buf + (W64.of_int 8));
+          lEN <- (lEN - 8);
+          (buf, lEN, tRAIL, t64) <@ __mread_subu64 (buf, lEN, tRAIL);
+          w <- (VPINSR_2u64 w t64 (W8.of_int 1));
+        } else {
+          (buf, lEN, tRAIL, t64) <@ __mread_subu64 (buf, lEN, tRAIL);
+          w <- (zeroextu128 t64);
+        }
+      }
+    }
+    return (buf, lEN, tRAIL, w);
+  }
+  proc __mread_subu256 (buf:W64.t, lEN:int, tRAIL:int) : W64.t * int * int *
+                                                         W256.t = {
+    var w:W256.t;
+    var t128_1:W128.t;
+    var t128_0:W128.t;
+    if (((lEN <= 0) /\ (tRAIL = 0))) {
+      w <- (set0_256);
+    } else {
+      if ((32 <= lEN)) {
+        w <- (loadW256 Glob.mem (W64.to_uint (buf + (W64.of_int 0))));
+        buf <- (buf + (W64.of_int 32));
+        lEN <- (lEN - 32);
+      } else {
+        if ((16 <= lEN)) {
+          t128_0 <- (loadW128 Glob.mem (W64.to_uint (buf + (W64.of_int 0))));
+          buf <- (buf + (W64.of_int 16));
+          lEN <- (lEN - 16);
+          (buf, lEN, tRAIL, t128_1) <@ __mread_subu128 (buf, lEN, tRAIL);
+          w <-
+          (W256.of_int
+          (((W128.to_uint t128_0) %% (2 ^ 128)) +
+          ((2 ^ 128) * (W128.to_uint t128_1))));
+        } else {
+          t128_1 <- (set0_128);
+          (buf, lEN, tRAIL, t128_0) <@ __mread_subu128 (buf, lEN, tRAIL);
+          w <-
+          (W256.of_int
+          (((W128.to_uint t128_0) %% (2 ^ 128)) +
+          ((2 ^ 128) * (W128.to_uint t128_1))));
+        }
+      }
+    }
+    return (buf, lEN, tRAIL, w);
+  }
+  proc __mwrite_subu64 (buf:W64.t, lEN:int, w:W64.t) : W64.t * int = {
+    
+    if ((0 < lEN)) {
+      if ((8 <= lEN)) {
+        Glob.mem <-
+        (storeW64 Glob.mem (W64.to_uint (buf + (W64.of_int 0))) w);
+        buf <- (buf + (W64.of_int 8));
+        lEN <- (lEN - 8);
+      } else {
+        if ((4 <= lEN)) {
+          Glob.mem <-
+          (storeW32 Glob.mem (W64.to_uint (buf + (W64.of_int 0)))
+          (truncateu32 w));
+          w <- (w `>>` (W8.of_int 32));
+          buf <- (buf + (W64.of_int 4));
+          lEN <- (lEN - 4);
+        } else {
+          
+        }
+        if ((2 <= lEN)) {
+          Glob.mem <-
+          (storeW16 Glob.mem (W64.to_uint (buf + (W64.of_int 0)))
+          (truncateu16 w));
+          w <- (w `>>` (W8.of_int 16));
+          buf <- (buf + (W64.of_int 2));
+          lEN <- (lEN - 2);
+        } else {
+          
+        }
+        if ((1 <= lEN)) {
+          Glob.mem <-
+          (storeW8 Glob.mem (W64.to_uint (buf + (W64.of_int 0)))
+          (truncateu8 w));
+          buf <- (buf + (W64.of_int 1));
+          lEN <- (lEN - 1);
+        } else {
+          
+        }
+      }
+    } else {
+      
+    }
+    return (buf, lEN);
+  }
+  proc __mwrite_subu128 (buf:W64.t, lEN:int, w:W128.t) : W64.t * int = {
+    var t64:W64.t;
+    if ((0 < lEN)) {
+      if ((16 <= lEN)) {
+        Glob.mem <-
+        (storeW128 Glob.mem (W64.to_uint (buf + (W64.of_int 0))) w);
+        buf <- (buf + (W64.of_int 16));
+        lEN <- (lEN - 16);
+      } else {
+        if ((8 <= lEN)) {
+          Glob.mem <-
+          (storeW64 Glob.mem (W64.to_uint (buf + (W64.of_int 0)))
+          (MOVV_64 (truncateu64 w)));
+          buf <- (buf + (W64.of_int 8));
+          lEN <- (lEN - 8);
+          w <- (VPUNPCKH_2u64 w w);
+        } else {
+          
+        }
+        t64 <- (truncateu64 w);
+        (buf, lEN) <@ __mwrite_subu64 (buf, lEN, t64);
+      }
+    } else {
+      
+    }
+    return (buf, lEN);
+  }
+  proc __mwrite_subu256 (buf:W64.t, lEN:int, w:W256.t) : W64.t * int = {
+    var t128:W128.t;
+    if ((0 < lEN)) {
+      if ((32 <= lEN)) {
+        Glob.mem <-
+        (storeW256 Glob.mem (W64.to_uint (buf + (W64.of_int 0))) w);
+        buf <- (buf + (W64.of_int 32));
+        lEN <- (lEN - 32);
+      } else {
+        if ((16 <= lEN)) {
+          Glob.mem <-
+          (storeW128 Glob.mem (W64.to_uint (buf + (W64.of_int 0)))
+          (truncateu128 w));
+          buf <- (buf + (W64.of_int 16));
+          lEN <- (lEN - 16);
+          t128 <- (VEXTRACTI128 w (W8.of_int 1));
+        } else {
+          t128 <- (truncateu128 w);
+        }
+        (buf, lEN) <@ __mwrite_subu128 (buf, lEN, t128);
+      }
+    } else {
+      
+    }
+    return (buf, lEN);
+  }
+  proc __addstate_imem_ref (st:W64.t Array25.t, aT:int, buf:W64.t, lEN:int,
+                            tRAILB:int) : W64.t Array25.t * int * W64.t = {
+    var aLL:int;
+    var lO:int;
+    var at:W64.t;
+    var t:W64.t;
+    var  _0:int;
+    var  _1:int;
+    var  _2:int;
+    var  _3:int;
+    var  _4:int;
+    var  _5:int;
+    aLL <- (aT + lEN);
+    lO <- (aT %% 8);
+    at <- (W64.of_int (aT %/ 8));
+    if ((0 < lO)) {
+      if (((lO + lEN) < 8)) {
+        if ((tRAILB <> 0)) {
+          aLL <- (aLL + 1);
+        } else {
+          
+        }
+        (buf,  _2,  _3, t) <@ __mread_subu64 (buf, lEN, tRAILB);
+        t <- (t `<<` (W8.of_int (8 * lO)));
+        t <- (t `^` st.[(W64.to_uint at)]);
+        st.[(W64.to_uint at)] <- t;
+        lO <- 0;
+        aT <- 0;
+        lEN <- 0;
+        tRAILB <- 0;
+      } else {
+        if ((8 <= lEN)) {
+          t <- (loadW64 Glob.mem (W64.to_uint (buf + (W64.of_int 0))));
+          buf <- (buf + (W64.of_int (8 - lO)));
+        } else {
+          (buf,  _0,  _1, t) <@ __mread_subu64 (buf, (8 - lO), tRAILB);
+        }
+        lEN <- (lEN - (8 - lO));
+        aT <- (aT + (8 - lO));
+        t <- (t `<<` (W8.of_int (8 * lO)));
+        t <- (t `^` st.[(W64.to_uint at)]);
+        st.[(W64.to_uint at)] <- t;
+        at <- (at + (W64.of_int 1));
+      }
+    } else {
+      
+    }
+    if ((8 <= lEN)) {
+      while ((at \ult (W64.of_int ((aT %/ 8) + (lEN %/ 8))))) {
+        t <- (loadW64 Glob.mem (W64.to_uint (buf + (W64.of_int 0))));
+        buf <- (buf + (W64.of_int 8));
+        t <- (t `^` st.[(W64.to_uint at)]);
+        st.[(W64.to_uint at)] <- t;
+        at <- (at + (W64.of_int 1));
+      }
+      lEN <- ((aT + lEN) %% 8);
+    } else {
+      
+    }
+    lO <- ((aT + lEN) %% 8);
+    if (((0 < lO) \/ (tRAILB <> 0))) {
+      (buf,  _4,  _5, t) <@ __mread_subu64 (buf, lO, tRAILB);
+      if ((tRAILB <> 0)) {
+        aLL <- (aLL + 1);
+        tRAILB <- 0;
+      } else {
+        
+      }
+      t <- (t `^` st.[(W64.to_uint at)]);
+      st.[(W64.to_uint at)] <- t;
+    } else {
+      
+    }
+    return (st, aLL, buf);
+  }
+  proc __absorb_imem_ref (st:W64.t Array25.t, aT:int, buf:W64.t, lEN:int,
+                          rATE8:int, tRAILB:int) : W64.t Array25.t * int *
+                                                   W64.t = {
+    var aLL:int;
+    var iTERS:int;
+    var i:W64.t;
+    var  _0:int;
+    var  _1:int;
+    aLL <- (aT + lEN);
+    if (((aT + lEN) < rATE8)) {
+      (st, aT, buf) <@ __addstate_imem_ref (st, aT, buf, lEN, tRAILB);
+      if ((tRAILB <> 0)) {
+        st <@ __addratebit_ref (st, rATE8);
+      } else {
+        
+      }
+    } else {
+      if ((aT <> 0)) {
+        (st,  _0, buf) <@ __addstate_imem_ref (st, aT, buf, (rATE8 - aT), 0);
+        lEN <- (lEN - (rATE8 - aT));
+        (* Erased call to spill *)
+        st <@ _keccakf1600_ref (st);
+        (* Erased call to unspill *)
+        aT <- 0;
+      } else {
+        
+      }
+      iTERS <- (lEN %/ rATE8);
+      i <- (W64.of_int 0);
+      while ((i \ult (W64.of_int iTERS))) {
+        (st,  _1, buf) <@ __addstate_imem_ref (st, 0, buf, rATE8, 0);
+        (* Erased call to spill *)
+        st <@ _keccakf1600_ref (st);
+        (* Erased call to unspill *)
+        i <- (i + (W64.of_int 1));
+      }
+      lEN <- (aLL %% rATE8);
+      (st, aT, buf) <@ __addstate_imem_ref (st, 0, buf, lEN, tRAILB);
+      if ((tRAILB <> 0)) {
+        st <@ __addratebit_ref (st, rATE8);
+      } else {
+        
+      }
+    }
+    return (st, aT, buf);
+  }
+  proc __dumpstate_imem_ref (buf:W64.t, lEN:int, st:W64.t Array25.t) : W64.t = {
+    var i:W64.t;
+    var t:W64.t;
+    var  _0:int;
+    i <- (W64.of_int 0);
+    while ((i \slt (W64.of_int (lEN %/ 8)))) {
+      t <- st.[(W64.to_uint i)];
+      i <- (i + (W64.of_int 1));
+      Glob.mem <- (storeW64 Glob.mem (W64.to_uint (buf + (W64.of_int 0))) t);
+      buf <- (buf + (W64.of_int 8));
+    }
+    if ((0 < (lEN %% 8))) {
+      t <- st.[(W64.to_uint i)];
+      (buf,  _0) <@ __mwrite_subu64 (buf, (lEN %% 8), t);
+    } else {
+      
+    }
+    return buf;
+  }
+  proc __squeeze_imem_ref (buf:W64.t, lEN:int, st:W64.t Array25.t, rATE8:int) : 
+  W64.t * W64.t Array25.t = {
+    var iTERS:int;
+    var lO:int;
+    var i:W64.t;
+    iTERS <- (lEN %/ rATE8);
+    lO <- (lEN %% rATE8);
+    if ((0 < lEN)) {
+      if ((0 < iTERS)) {
+        i <- (W64.of_int 0);
+        while ((i \ult (W64.of_int iTERS))) {
+          (* Erased call to spill *)
+          st <@ _keccakf1600_ref (st);
+          (* Erased call to unspill *)
+          buf <@ __dumpstate_imem_ref (buf, rATE8, st);
+          i <- (i + (W64.of_int 1));
+        }
+      } else {
+        
+      }
+      if ((0 < lO)) {
+        (* Erased call to spill *)
+        st <@ _keccakf1600_ref (st);
+        (* Erased call to unspill *)
+        buf <@ __dumpstate_imem_ref (buf, lO, st);
+      } else {
+        
+      }
+    } else {
+      
+    }
+    return (buf, st);
+  }
+}.
