proof/extracted/Jazz_ref_ASIZE.ec
@@ -1,0 +1,729 @@
+require import AllCore IntDiv CoreMap List Distr.
+
+from Jasmin require import JModel_x86.
+
+import SLH64.
+
+require import
+Array5 Array24 Array25 Array999 WArray40 WArray192 WArray200 WArray999.
+
+abbrev kECCAK1600_RC =
+(Array24.of_list witness
+[(W64.of_int 1); (W64.of_int 32898); (W64.of_int (-9223372036854742902));
+(W64.of_int (-9223372034707259392)); (W64.of_int 32907);
+(W64.of_int 2147483649); (W64.of_int (-9223372034707259263));
+(W64.of_int (-9223372036854743031)); (W64.of_int 138); (W64.of_int 136);
+(W64.of_int 2147516425); (W64.of_int 2147483658); (W64.of_int 2147516555);
+(W64.of_int (-9223372036854775669)); (W64.of_int (-9223372036854742903));
+(W64.of_int (-9223372036854743037)); (W64.of_int (-9223372036854743038));
+(W64.of_int (-9223372036854775680)); (W64.of_int 32778);
+(W64.of_int (-9223372034707292150)); (W64.of_int (-9223372034707259263));
+(W64.of_int (-9223372036854742912)); (W64.of_int 2147483649);
+(W64.of_int (-9223372034707259384))]).
+
+module M = {
+  proc __ANDN_64 (a:W64.t, b:W64.t) : W64.t = {
+    var t:W64.t;
+    t <- a;
+    t <- (invw t);
+    t <- (t `&` b);
+    return t;
+  }
+  proc keccakf1600_index (x:int, y:int) : int = {
+    var r:int;
+    r <- ((x %% 5) + (5 * (y %% 5)));
+    return r;
+  }
+  proc keccakf1600_rho_offsets (i:int) : int = {
+    var aux:int;
+    var r:int;
+    var x:int;
+    var y:int;
+    var t:int;
+    var z:int;
+    r <- 0;
+    x <- 1;
+    y <- 0;
+    t <- 0;
+    while ((t < 24)) {
+      if ((i = (x + (5 * y)))) {
+        r <- ((((t + 1) * (t + 2)) %/ 2) %% 64);
+      } else {
+        
+      }
+      z <- (((2 * x) + (3 * y)) %% 5);
+      x <- y;
+      y <- z;
+      t <- (t + 1);
+    }
+    return r;
+  }
+  proc keccakf1600_rhotates (x:int, y:int) : int = {
+    var r:int;
+    var i:int;
+    i <@ keccakf1600_index (x, y);
+    r <@ keccakf1600_rho_offsets (i);
+    return r;
+  }
+  proc __rol_u64_ref (x:W64.t, i:int) : W64.t = {
+    var  _0:bool;
+    var  _1:bool;
+    if ((i <> 0)) {
+      ( _0,  _1, x) <- (ROL_64 x (W8.of_int i));
+    } else {
+      
+    }
+    return x;
+  }
+  proc __theta_sum_ref (a:W64.t Array25.t) : W64.t Array5.t = {
+    var aux:int;
+    var c:W64.t Array5.t;
+    var x:int;
+    var y:int;
+    c <- witness;
+    x <- 0;
+    while ((x < 5)) {
+      c.[x] <- a.[(x + 0)];
+      x <- (x + 1);
+    }
+    y <- 1;
+    while ((y < 5)) {
+      x <- 0;
+      while ((x < 5)) {
+        c.[x] <- (c.[x] `^` a.[(x + (y * 5))]);
+        x <- (x + 1);
+      }
+      y <- (y + 1);
+    }
+    return c;
+  }
+  proc __theta_rol_ref (c:W64.t Array5.t) : W64.t Array5.t = {
+    var aux:int;
+    var aux_0:W64.t;
+    var d:W64.t Array5.t;
+    var x:int;
+    d <- witness;
+    x <- 0;
+    while ((x < 5)) {
+      d.[x] <- c.[((x + 1) %% 5)];
+      aux_0 <@ __rol_u64_ref (d.[x], 1);
+      d.[x] <- aux_0;
+      d.[x] <- (d.[x] `^` c.[(((x - 1) + 5) %% 5)]);
+      x <- (x + 1);
+    }
+    return d;
+  }
+  proc __rol_sum_ref (a:W64.t Array25.t, d:W64.t Array5.t, y:int) : W64.t Array5.t = {
+    var aux:int;
+    var aux_0:W64.t;
+    var b:W64.t Array5.t;
+    var x:int;
+    var x_:int;
+    var y_:int;
+    var r:int;
+    b <- witness;
+    x <- 0;
+    while ((x < 5)) {
+      x_ <- ((x + (3 * y)) %% 5);
+      y_ <- x;
+      r <@ keccakf1600_rhotates (x_, y_);
+      b.[x] <- a.[(x_ + (y_ * 5))];
+      b.[x] <- (b.[x] `^` d.[x_]);
+      aux_0 <@ __rol_u64_ref (b.[x], r);
+      b.[x] <- aux_0;
+      x <- (x + 1);
+    }
+    return b;
+  }
+  proc __set_row_ref (e:W64.t Array25.t, b:W64.t Array5.t, y:int, s_rc:W64.t) : 
+  W64.t Array25.t = {
+    var aux:int;
+    var x:int;
+    var x1:int;
+    var x2:int;
+    var t:W64.t;
+    x <- 0;
+    while ((x < 5)) {
+      x1 <- ((x + 1) %% 5);
+      x2 <- ((x + 2) %% 5);
+      t <@ __ANDN_64 (b.[x1], b.[x2]);
+      t <- (t `^` b.[x]);
+      if (((x = 0) /\ (y = 0))) {
+        t <- (t `^` s_rc);
+      } else {
+        
+      }
+      e.[(x + (y * 5))] <- t;
+      x <- (x + 1);
+    }
+    return e;
+  }
+  proc __round_ref (e:W64.t Array25.t, a:W64.t Array25.t, s_rc:W64.t) : 
+  W64.t Array25.t = {
+    var aux:int;
+    var c:W64.t Array5.t;
+    var d:W64.t Array5.t;
+    var y:int;
+    var b:W64.t Array5.t;
+    b <- witness;
+    c <- witness;
+    d <- witness;
+    c <@ __theta_sum_ref (a);
+    d <@ __theta_rol_ref (c);
+    y <- 0;
+    while ((y < 5)) {
+      b <@ __rol_sum_ref (a, d, y);
+      e <@ __set_row_ref (e, b, y, s_rc);
+      y <- (y + 1);
+    }
+    return e;
+  }
+  proc __keccakf1600_ref (a:W64.t Array25.t) : W64.t Array25.t = {
+    var rC:W64.t Array24.t;
+    var s_RC:W64.t Array24.t;
+    var s_e:W64.t Array25.t;
+    var e:W64.t Array25.t;
+    var c:W64.t;
+    var s_c:W64.t;
+    var rc:W64.t;
+    var s_rc:W64.t;
+    rC <- witness;
+    e <- witness;
+    s_RC <- witness;
+    s_e <- witness;
+    rC <- kECCAK1600_RC;
+    s_RC <- rC;
+    e <- s_e;
+    c <- (W64.of_int 0);
+    s_c <- c;
+    rC <- s_RC;
+    rc <- rC.[(W64.to_uint c)];
+    s_rc <- rc;
+    e <@ __round_ref (e, a, s_rc);
+    rC <- s_RC;
+    rc <- rC.[((W64.to_uint c) + 1)];
+    s_rc <- rc;
+    a <@ __round_ref (a, e, s_rc);
+    c <- s_c;
+    c <- (c + (W64.of_int 2));
+    while ((c \ult (W64.of_int (24 - 1)))) {
+      s_c <- c;
+      rC <- s_RC;
+      rc <- rC.[(W64.to_uint c)];
+      s_rc <- rc;
+      e <@ __round_ref (e, a, s_rc);
+      rC <- s_RC;
+      rc <- rC.[((W64.to_uint c) + 1)];
+      s_rc <- rc;
+      a <@ __round_ref (a, e, s_rc);
+      c <- s_c;
+      c <- (c + (W64.of_int 2));
+    }
+    return a;
+  }
+  proc _keccakf1600_ref (a:W64.t Array25.t) : W64.t Array25.t = {
+    
+    a <@ __keccakf1600_ref (a);
+    return a;
+  }
+  proc _keccakf1600_ref_ (a:W64.t Array25.t) : W64.t Array25.t = {
+    
+    a <- a;
+    a <@ _keccakf1600_ref (a);
+    a <- a;
+    return a;
+  }
+  proc __state_init_ref (st:W64.t Array25.t) : W64.t Array25.t = {
+    var z64:W64.t;
+    var i:W64.t;
+    z64 <- (W64.of_int 0);
+    i <- (W64.of_int 0);
+    while ((i \ult (W64.of_int 25))) {
+      st.[(W64.to_uint i)] <- z64;
+      i <- (i + (W64.of_int 1));
+    }
+    return st;
+  }
+  proc __addratebit_ref (st:W64.t Array25.t, rATE8:int) : W64.t Array25.t = {
+    var t64:W64.t;
+    t64 <- (W64.of_int 1);
+    t64 <- (t64 `<<` (W8.of_int (((8 * rATE8) - 1) %% 64)));
+    t64 <- (t64 `^` st.[((rATE8 - 1) %/ 8)]);
+    st.[((rATE8 - 1) %/ 8)] <- t64;
+    return st;
+  }
+  proc __aread_subu64 (buf:W8.t Array999.t, offset:W64.t, dELTA:int, lEN:int,
+                       tRAIL:int) : int * int * int * W64.t = {
+    var w:W64.t;
+    var iLEN:int;
+    var t16:W64.t;
+    var t8:W64.t;
+    iLEN <- lEN;
+    if ((lEN <= 0)) {
+      w <- (W64.of_int (tRAIL %% 256));
+      tRAIL <- 0;
+    } else {
+      if ((8 <= lEN)) {
+        w <-
+        (get64_direct (WArray999.init8 (fun i => buf.[i]))
+        (W64.to_uint (offset + (W64.of_int dELTA))));
+        dELTA <- (dELTA + 8);
+        lEN <- (lEN - 8);
+      } else {
+        if ((4 <= lEN)) {
+          w <-
+          (zeroextu64
+          (get32_direct (WArray999.init8 (fun i => buf.[i]))
+          (W64.to_uint (offset + (W64.of_int dELTA)))));
+          dELTA <- (dELTA + 4);
+          lEN <- (lEN - 4);
+        } else {
+          w <- (W64.of_int 0);
+        }
+        if ((2 <= lEN)) {
+          t16 <-
+          (zeroextu64
+          (get16_direct (WArray999.init8 (fun i => buf.[i]))
+          (W64.to_uint (offset + (W64.of_int dELTA)))));
+          dELTA <- (dELTA + 2);
+          lEN <- (lEN - 2);
+        } else {
+          t16 <- (W64.of_int 0);
+        }
+        if (((1 <= lEN) \/ ((tRAIL %% 256) <> 0))) {
+          if ((1 <= lEN)) {
+            t8 <-
+            (zeroextu64
+            (get8_direct (WArray999.init8 (fun i => buf.[i]))
+            (W64.to_uint (offset + (W64.of_int dELTA)))));
+            if (((tRAIL %% 256) <> 0)) {
+              t8 <- (t8 `|` (W64.of_int (256 * (tRAIL %% 256))));
+            } else {
+              
+            }
+            dELTA <- (dELTA + 1);
+            lEN <- (lEN - 1);
+          } else {
+            t8 <- (W64.of_int (tRAIL %% 256));
+          }
+          tRAIL <- 0;
+          t8 <- (t8 `<<` (W8.of_int (8 * (2 * ((iLEN %/ 2) %% 2)))));
+          t16 <- (t16 `|` t8);
+        } else {
+          
+        }
+        t16 <- (t16 `<<` (W8.of_int (8 * (4 * ((iLEN %/ 4) %% 2)))));
+        w <- (w `|` t16);
+      }
+    }
+    return (dELTA, lEN, tRAIL, w);
+  }
+  proc __aread_bcast_4subu64 (buf:W8.t Array999.t, offset:W64.t, dELTA:int,
+                              lEN:int, tRAIL:int) : int * int * int * W256.t = {
+    var w:W256.t;
+    var t64:W64.t;
+    var t128:W128.t;
+    if (((lEN <= 0) /\ ((tRAIL %% 256) = 0))) {
+      w <- (set0_256);
+    } else {
+      if ((8 <= lEN)) {
+        w <-
+        (VPBROADCAST_4u64
+        (get64_direct (WArray999.init8 (fun i => buf.[i]))
+        (W64.to_uint (offset + (W64.of_int dELTA)))));
+        dELTA <- (dELTA + 8);
+        lEN <- (lEN - 8);
+      } else {
+        (dELTA, lEN, tRAIL, t64) <@ __aread_subu64 (buf, offset, dELTA, 
+        lEN, tRAIL);
+        t128 <- (zeroextu128 t64);
+        w <- (VPBROADCAST_4u64 (truncateu64 t128));
+      }
+    }
+    return (dELTA, lEN, tRAIL, w);
+  }
+  proc __aread_subu128 (buf:W8.t Array999.t, offset:W64.t, dELTA:int,
+                        lEN:int, tRAIL:int) : int * int * int * W128.t = {
+    var w:W128.t;
+    var t64:W64.t;
+    if (((lEN <= 0) /\ ((tRAIL %% 256) = 0))) {
+      w <- (set0_128);
+    } else {
+      if ((16 <= lEN)) {
+        w <-
+        (get128_direct (WArray999.init8 (fun i => buf.[i]))
+        (W64.to_uint (offset + (W64.of_int dELTA))));
+        dELTA <- (dELTA + 16);
+        lEN <- (lEN - 16);
+      } else {
+        if ((8 <= lEN)) {
+          w <-
+          (VMOV_64
+          (get64_direct (WArray999.init8 (fun i => buf.[i]))
+          (W64.to_uint (offset + (W64.of_int dELTA)))));
+          dELTA <- (dELTA + 8);
+          lEN <- (lEN - 8);
+          (dELTA, lEN, tRAIL, t64) <@ __aread_subu64 (buf, offset, dELTA,
+          lEN, tRAIL);
+          w <- (VPINSR_2u64 w t64 (W8.of_int 1));
+        } else {
+          (dELTA, lEN, tRAIL, t64) <@ __aread_subu64 (buf, offset, dELTA,
+          lEN, tRAIL);
+          w <- (zeroextu128 t64);
+        }
+      }
+    }
+    return (dELTA, lEN, tRAIL, w);
+  }
+  proc __aread_subu256 (buf:W8.t Array999.t, offset:W64.t, dELTA:int,
+                        lEN:int, tRAIL:int) : int * int * int * W256.t = {
+    var w:W256.t;
+    var t128_1:W128.t;
+    var t128_0:W128.t;
+    if (((lEN <= 0) /\ ((tRAIL %% 256) = 0))) {
+      w <- (set0_256);
+    } else {
+      if ((32 <= lEN)) {
+        w <-
+        (get256_direct (WArray999.init8 (fun i => buf.[i]))
+        (W64.to_uint (offset + (W64.of_int dELTA))));
+        dELTA <- (dELTA + 32);
+        lEN <- (lEN - 32);
+      } else {
+        if ((16 <= lEN)) {
+          t128_0 <-
+          (get128_direct (WArray999.init8 (fun i => buf.[i]))
+          (W64.to_uint (offset + (W64.of_int dELTA))));
+          dELTA <- (dELTA + 16);
+          lEN <- (lEN - 16);
+          (dELTA, lEN, tRAIL, t128_1) <@ __aread_subu128 (buf, offset, 
+          dELTA, lEN, tRAIL);
+          w <-
+          (W256.of_int
+          (((W128.to_uint t128_0) %% (2 ^ 128)) +
+          ((2 ^ 128) * (W128.to_uint t128_1))));
+        } else {
+          t128_1 <- (set0_128);
+          (dELTA, lEN, tRAIL, t128_0) <@ __aread_subu128 (buf, offset, 
+          dELTA, lEN, tRAIL);
+          w <-
+          (W256.of_int
+          (((W128.to_uint t128_0) %% (2 ^ 128)) +
+          ((2 ^ 128) * (W128.to_uint t128_1))));
+        }
+      }
+    }
+    return (dELTA, lEN, tRAIL, w);
+  }
+  proc __awrite_subu64 (buf:W8.t Array999.t, offset:W64.t, dELTA:int,
+                        lEN:int, w:W64.t) : W8.t Array999.t * int * int = {
+    
+    if ((0 < lEN)) {
+      if ((8 <= lEN)) {
+        buf <-
+        (Array999.init
+        (WArray999.get8
+        (WArray999.set64_direct (WArray999.init8 (fun i => buf.[i]))
+        (W64.to_uint (offset + (W64.of_int dELTA))) w)));
+        dELTA <- (dELTA + 8);
+        lEN <- (lEN - 8);
+      } else {
+        if ((4 <= lEN)) {
+          buf <-
+          (Array999.init
+          (WArray999.get8
+          (WArray999.set32_direct (WArray999.init8 (fun i => buf.[i]))
+          (W64.to_uint (offset + (W64.of_int dELTA))) (truncateu32 w))));
+          w <- (w `>>` (W8.of_int 32));
+          dELTA <- (dELTA + 4);
+          lEN <- (lEN - 4);
+        } else {
+          
+        }
+        if ((2 <= lEN)) {
+          buf <-
+          (Array999.init
+          (WArray999.get8
+          (WArray999.set16_direct (WArray999.init8 (fun i => buf.[i]))
+          (W64.to_uint (offset + (W64.of_int dELTA))) (truncateu16 w))));
+          w <- (w `>>` (W8.of_int 16));
+          dELTA <- (dELTA + 2);
+          lEN <- (lEN - 2);
+        } else {
+          
+        }
+        if ((1 <= lEN)) {
+          buf <-
+          (Array999.init
+          (WArray999.get8
+          (WArray999.set8_direct (WArray999.init8 (fun i => buf.[i]))
+          (W64.to_uint (offset + (W64.of_int dELTA))) (truncateu8 w))));
+          dELTA <- (dELTA + 1);
+          lEN <- (lEN - 1);
+        } else {
+          
+        }
+      }
+    } else {
+      
+    }
+    return (buf, dELTA, lEN);
+  }
+  proc __awrite_subu128 (buf:W8.t Array999.t, offset:W64.t, dELTA:int,
+                         lEN:int, w:W128.t) : W8.t Array999.t * int * int = {
+    var t64:W64.t;
+    if ((0 < lEN)) {
+      if ((16 <= lEN)) {
+        buf <-
+        (Array999.init
+        (WArray999.get8
+        (WArray999.set128_direct (WArray999.init8 (fun i => buf.[i]))
+        (W64.to_uint (offset + (W64.of_int dELTA))) w)));
+        dELTA <- (dELTA + 16);
+        lEN <- (lEN - 16);
+      } else {
+        if ((8 <= lEN)) {
+          buf <-
+          (Array999.init
+          (WArray999.get8
+          (WArray999.set64_direct (WArray999.init8 (fun i => buf.[i]))
+          (W64.to_uint (offset + (W64.of_int dELTA)))
+          (MOVV_64 (truncateu64 w)))));
+          dELTA <- (dELTA + 8);
+          lEN <- (lEN - 8);
+          w <- (VPUNPCKH_2u64 w w);
+        } else {
+          
+        }
+        t64 <- (truncateu64 w);
+        (buf, dELTA, lEN) <@ __awrite_subu64 (buf, offset, dELTA, lEN, t64);
+      }
+    } else {
+      
+    }
+    return (buf, dELTA, lEN);
+  }
+  proc __awrite_subu256 (buf:W8.t Array999.t, offset:W64.t, dELTA:int,
+                         lEN:int, w:W256.t) : W8.t Array999.t * int * int = {
+    var t128:W128.t;
+    if ((0 < lEN)) {
+      if ((32 <= lEN)) {
+        buf <-
+        (Array999.init
+        (WArray999.get8
+        (WArray999.set256_direct (WArray999.init8 (fun i => buf.[i]))
+        (W64.to_uint (offset + (W64.of_int dELTA))) w)));
+        dELTA <- (dELTA + 32);
+        lEN <- (lEN - 32);
+      } else {
+        if ((16 <= lEN)) {
+          buf <-
+          (Array999.init
+          (WArray999.get8
+          (WArray999.set128_direct (WArray999.init8 (fun i => buf.[i]))
+          (W64.to_uint (offset + (W64.of_int dELTA))) (truncateu128 w))));
+          dELTA <- (dELTA + 16);
+          lEN <- (lEN - 16);
+          t128 <- (VEXTRACTI128 w (W8.of_int 1));
+        } else {
+          t128 <- (truncateu128 w);
+        }
+        (buf, dELTA, lEN) <@ __awrite_subu128 (buf, offset, dELTA, lEN,
+        t128);
+      }
+    } else {
+      
+    }
+    return (buf, dELTA, lEN);
+  }
+  proc __addstate_array_ref (st:W64.t Array25.t, aT:int, buf:W8.t Array999.t,
+                             offset:W64.t, lEN:int, tRAILB:int) : W64.t Array25.t *
+                                                                  int * W64.t = {
+    var aLL:int;
+    var lO:int;
+    var at:W64.t;
+    var dELTA:int;
+    var t:W64.t;
+    var  _0:int;
+    var  _1:int;
+    var  _2:int;
+    var  _3:int;
+    var  _4:int;
+    var  _5:int;
+    aLL <- (aT + lEN);
+    lO <- (aT %% 8);
+    at <- (W64.of_int (aT %/ 8));
+    dELTA <- 0;
+    if ((0 < lO)) {
+      if (((lO + lEN) < 8)) {
+        if ((tRAILB <> 0)) {
+          aLL <- (aLL + 1);
+        } else {
+          
+        }
+        (dELTA,  _2,  _3, t) <@ __aread_subu64 (buf, offset, dELTA, lEN,
+        tRAILB);
+        t <- (t `<<` (W8.of_int (8 * lO)));
+        t <- (t `^` st.[(W64.to_uint at)]);
+        st.[(W64.to_uint at)] <- t;
+        lO <- 0;
+        aT <- 0;
+        lEN <- 0;
+        tRAILB <- 0;
+      } else {
+        if ((8 <= lEN)) {
+          t <-
+          (get64_direct (WArray999.init8 (fun i => buf.[i]))
+          (W64.to_uint (offset + (W64.of_int dELTA))));
+          offset <- (offset + (W64.of_int (8 - lO)));
+        } else {
+          (dELTA,  _0,  _1, t) <@ __aread_subu64 (buf, offset, dELTA,
+          (8 - lO), tRAILB);
+        }
+        lEN <- (lEN - (8 - lO));
+        aT <- (aT + (8 - lO));
+        t <- (t `<<` (W8.of_int (8 * lO)));
+        t <- (t `^` st.[(W64.to_uint at)]);
+        st.[(W64.to_uint at)] <- t;
+        at <- (at + (W64.of_int 1));
+      }
+    } else {
+      
+    }
+    offset <- (offset + (W64.of_int dELTA));
+    dELTA <- 0;
+    if ((8 <= lEN)) {
+      while ((at \ult (W64.of_int ((aT %/ 8) + (lEN %/ 8))))) {
+        t <-
+        (get64_direct (WArray999.init8 (fun i => buf.[i]))
+        (W64.to_uint offset));
+        t <- (t `^` st.[(W64.to_uint at)]);
+        st.[(W64.to_uint at)] <- t;
+        at <- (at + (W64.of_int 1));
+      }
+      lEN <- ((aT + lEN) %% 8);
+    } else {
+      
+    }
+    lO <- ((aT + lEN) %% 8);
+    if (((0 < lO) \/ (tRAILB <> 0))) {
+      (dELTA,  _4,  _5, t) <@ __aread_subu64 (buf, offset, dELTA, lO,
+      tRAILB);
+      offset <- (offset + (W64.of_int dELTA));
+      if ((tRAILB <> 0)) {
+        aLL <- (aLL + 1);
+        tRAILB <- 0;
+      } else {
+        
+      }
+      t <- (t `^` st.[(W64.to_uint at)]);
+      st.[(W64.to_uint at)] <- t;
+    } else {
+      
+    }
+    return (st, aLL, offset);
+  }
+  proc __absorb_array_ref (st:W64.t Array25.t, aT:int, buf:W8.t Array999.t,
+                           offset:W64.t, lEN:int, rATE8:int, tRAILB:int) : 
+  W64.t Array25.t * int * W64.t = {
+    var aLL:int;
+    var iTERS:int;
+    var i:W64.t;
+    var  _0:int;
+    var  _1:int;
+    aLL <- (aT + lEN);
+    if (((aT + lEN) < rATE8)) {
+      (st, aT, offset) <@ __addstate_array_ref (st, aT, buf, offset, 
+      lEN, tRAILB);
+      if ((tRAILB <> 0)) {
+        st <@ __addratebit_ref (st, rATE8);
+      } else {
+        
+      }
+    } else {
+      if ((aT <> 0)) {
+        (st,  _0, offset) <@ __addstate_array_ref (st, aT, buf, offset,
+        (rATE8 - aT), 0);
+        lEN <- (lEN - (rATE8 - aT));
+        st <@ _keccakf1600_ref (st);
+        aT <- 0;
+      } else {
+        
+      }
+      iTERS <- (lEN %/ rATE8);
+      i <- (W64.of_int 0);
+      while ((i \ult (W64.of_int iTERS))) {
+        (st,  _1, offset) <@ __addstate_array_ref (st, 0, buf, offset, 
+        rATE8, 0);
+        st <@ _keccakf1600_ref (st);
+        i <- (i + (W64.of_int 1));
+      }
+      lEN <- (aLL %% rATE8);
+      (st, aT, offset) <@ __addstate_array_ref (st, 0, buf, offset, lEN,
+      tRAILB);
+      if ((tRAILB <> 0)) {
+        st <@ __addratebit_ref (st, rATE8);
+      } else {
+        
+      }
+    }
+    return (st, aT, offset);
+  }
+  proc __dumpstate_array_ref (buf:W8.t Array999.t, offset:W64.t, lEN:int,
+                              st:W64.t Array25.t) : W8.t Array999.t * W64.t = {
+    var i:W64.t;
+    var t:W64.t;
+    var  _0:int;
+    var  _1:int;
+    i <- (W64.of_int 0);
+    while ((i \slt (W64.of_int (lEN %/ 8)))) {
+      t <- st.[(W64.to_uint i)];
+      buf <-
+      (Array999.init
+      (WArray999.get8
+      (WArray999.set64_direct (WArray999.init8 (fun i_0 => buf.[i_0]))
+      (W64.to_uint offset) t)));
+      i <- (i + (W64.of_int 1));
+      offset <- (offset + (W64.of_int 8));
+    }
+    if ((0 < (lEN %% 8))) {
+      t <- st.[(W64.to_uint i)];
+      (buf,  _0,  _1) <@ __awrite_subu64 (buf, offset, 0, (lEN %% 8), t);
+      offset <- (offset + (W64.of_int (lEN %% 8)));
+    } else {
+      
+    }
+    return (buf, offset);
+  }
+  proc __squeeze_array_ref (buf:W8.t Array999.t, offset:W64.t, lEN:int,
+                            st:W64.t Array25.t, rATE8:int) : W8.t Array999.t *
+                                                             W64.t *
+                                                             W64.t Array25.t = {
+    var iTERS:int;
+    var lO:int;
+    var i:W64.t;
+    iTERS <- (lEN %/ rATE8);
+    lO <- (lEN %% rATE8);
+    if ((0 < lEN)) {
+      if ((0 < iTERS)) {
+        i <- (W64.of_int 0);
+        while ((i \ult (W64.of_int iTERS))) {
+          st <@ _keccakf1600_ref (st);
+          (buf, offset) <@ __dumpstate_array_ref (buf, offset, rATE8, st);
+          i <- (i + (W64.of_int 1));
+        }
+      } else {
+        
+      }
+      if ((0 < lO)) {
+        st <@ _keccakf1600_ref (st);
+        (buf, offset) <@ __dumpstate_array_ref (buf, offset, lO, st);
+      } else {
+        
+      }
+    } else {
+      
+    }
+    return (buf, offset, st);
+  }
+}.
