proof/extracted/WArray999.ec
@@ -1,0 +1,3 @@
+from Jasmin require import JWord_array.
+
+clone export WArray as WArray999  with op size <- 999.
